Example proofs of constant-time behavior.

arm/proofs/bignum_copy.ml
@@ -7,7 +7,10 @@
 (* Copying (with truncation or extension) bignums                            *)
 (* ========================================================================= *)
 
-needs "arm/proofs/base.ml";;
+needs "arm/proofs/equiv.ml";;
+needs "common/relational_n.ml";;
+needs "common/bignum_n.ml";;
+needs "arm/proofs/arm_n.ml";;
 
 (**** print_literal_from_elf "arm/generic/bignum_copy.o";;
  ****)
@@ -39,6 +42,207 @@ let BIGNUM_COPY_EXEC = ARM_MK_EXEC_RULE bignum_copy_mc;;
 (* Correctness proof.                                                        *)
 (* ------------------------------------------------------------------------- *)
 
+let STEPS_LEMMA = prove(
+  `!n k. 4 * k + MIN n k + 6 = 3 + (1 + 5 * MIN n k) + 2 + 4 * (k - (MIN n k))`,
+  ARITH_TAC);;
+
+let ENUMERATEL = new_recursive_definition num_RECURSION
+  `(ENUMERATEL 0 (f:num->A list) = []) /\
+   (ENUMERATEL (SUC n) f = APPEND (f n) (ENUMERATEL n f))`;;
+
+let events = `\k z n x. APPEND
+  (ENUMERATEL (k - MIN n k) (\i. [EventStore (word_add z (word (8 * ((MIN n k) + i))))]))
+  (ENUMERATEL (MIN n k) (\i. [EventStore (word_add z (word (8 * i)));
+                              EventLoad (word_add x (word (8 * i)))]))`;;
+
+let BIGNUM_COPY_ALL = prove
+ (`?f_es. !k z n x a pc es.
+     nonoverlapping (word pc,0x40) (z,8 * val k) /\
+     (x = z \/ nonoverlapping (x,8 * MIN (val n) (val k)) (z,8 * val k))
+     ==> ensures_n arm
+           (\s. aligned_bytes_loaded s (word pc) bignum_copy_mc /\
+                read PC s = word pc /\
+                C_ARGUMENTS [k; z; n; x] s /\
+                bignum_from_memory (x,val n) s = a /\
+                read events s = es)
+           (\s. read PC s = word (pc + 0x3c) /\
+                bignum_from_memory (z,val k) s = lowdigits a (val k) /\
+                read events s = APPEND (f_es (val k) z (val n) x) es)
+           (MAYCHANGE [PC; X2; X4; X5] ,, MAYCHANGE SOME_FLAGS ,,
+            MAYCHANGE [memory :> bignum(z,val k)] ,,
+            MAYCHANGE [events])
+           (\s. 4 * val k + MIN (val n) (val k) + 6)`,
+  EXISTS_TAC events THEN
+  REWRITE_TAC[STEPS_LEMMA; NONOVERLAPPING_CLAUSES] THEN
+  REWRITE_TAC[C_ARGUMENTS; C_RETURN; SOME_FLAGS; fst BIGNUM_COPY_EXEC] THEN
+  W64_GEN_TAC `k:num` THEN X_GEN_TAC `z:int64` THEN
+  W64_GEN_TAC `n:num` THEN X_GEN_TAC `x:int64` THEN
+  MAP_EVERY X_GEN_TAC [`a:num`; `pc:num`; `es:armevent list`] THEN
+  DISCH_THEN(REPEAT_TCL CONJUNCTS_THEN ASSUME_TAC) THEN
+
+  (*** Simulate the initial computation of min(n,k) and then
+   *** recast the problem with n' = min(n,k) so we can assume
+   *** hereafter that n <= k. This makes life a bit easier since
+   *** otherwise n can actually be any number < 2^64 without
+   *** violating the preconditions.
+   ***)
+
+  ENSURES_N_SEQUENCE_TAC `pc + 0xc`
+   `\s. read X0 s = word k /\
+        read X1 s = z /\
+        read X2 s = word(MIN n k) /\
+        read X3 s = x /\
+        read X4 s = word 0 /\
+        bignum_from_memory (x,MIN n k) s = lowdigits a k /\
+        read events s = es` THEN
+  CONJ_TAC THENL
+   [REWRITE_TAC[GSYM LOWDIGITS_BIGNUM_FROM_MEMORY] THEN
+    ARM_SIM'_TAC BIGNUM_COPY_EXEC (1--3) THEN
+    REWRITE_TAC[ARITH_RULE `MIN n k = if k < n then k else n`] THEN
+    MESON_TAC[];
+    REPEAT(FIRST_X_ASSUM(MP_TAC o check (vfree_in `k:num` o concl))) THEN
+    POP_ASSUM_LIST(K ALL_TAC) THEN MP_TAC(ARITH_RULE `MIN n k <= k`) THEN
+    SPEC_TAC(`lowdigits a k`,`a:num`) THEN SPEC_TAC(`MIN n k`,`n:num`) THEN
+    REPEAT GEN_TAC THEN REPEAT DISCH_TAC THEN
+    VAL_INT64_TAC `n:num` THEN BIGNUM_RANGE'_TAC "n" "a"] THEN
+
+  (*** Break at the start of the padding stage ***)
+
+  ENSURES_N_SEQUENCE_TAC `pc + 0x24`
+   `\s. read X0 s = word k /\
+        read X1 s = z /\
+        read X4 s = word n /\
+        bignum_from_memory(z,n) s = a /\
+        read events s = APPEND (ENUMERATEL n (\i. CONS (EventStore (word_add z (word (8 * i)))) (CONS (EventLoad (word_add x (word (8 * i)))) []))) es` THEN
+  CONJ_TAC THENL
+   [ASM_CASES_TAC `n = 0` THENL
+     [ASM_REWRITE_TAC[BIGNUM_FROM_MEMORY_TRIVIAL] THEN
+      REWRITE_TAC[MESON[] `0 = a <=> a = 0`; ARITH_RULE `1 + 5 * 0 = 1`; ENUMERATEL; APPEND] THEN
+      ARM_SIM'_TAC BIGNUM_COPY_EXEC [1];
+      ALL_TAC] THEN
+
+    FIRST_ASSUM(MP_TAC o MATCH_MP (ONCE_REWRITE_RULE[IMP_CONJ]
+      NONOVERLAPPING_IMP_SMALL_2)) THEN
+    ANTS_TAC THENL [SIMPLE_ARITH_TAC; DISCH_TAC] THEN
+
+    (*** The main copying loop, in the case when n is nonzero ***)
+
+    ENSURES_N_WHILE_UP_TAC `n:num` `pc + 0x10` `pc + 0x1c`
+     `\i s. read X0 s = word k /\
+            read X1 s = z /\
+            read X2 s = word n /\
+            read X3 s = x /\
+            read X4 s = word i /\
+            bignum_from_memory(z,i) s = lowdigits a i /\
+            bignum_from_memory(word_add x (word(8 * i)),n - i) s = highdigits a i /\
+            read events s = APPEND (ENUMERATEL i (\j. [EventStore (word_add z (word (8 * j)));
+                                                       EventLoad (word_add x (word (8 * j)))])) es`
+      `(\i:num. 3)` `1` `2` `2` THEN
+    ASM_REWRITE_TAC[] THEN REPEAT CONJ_TAC THENL
+     [ARM_SIM'_TAC BIGNUM_COPY_EXEC [1] THEN
+      REWRITE_TAC[SUB_0; GSYM BIGNUM_FROM_MEMORY_BYTES; HIGHDIGITS_0] THEN
+      REWRITE_TAC[BIGNUM_FROM_MEMORY_TRIVIAL; MULT_CLAUSES; WORD_ADD_0] THEN
+      ASM_REWRITE_TAC[BIGNUM_FROM_MEMORY_BYTES; LOWDIGITS_0] THEN
+      REWRITE_TAC [ENUMERATEL; APPEND];
+      X_GEN_TAC `i:num` THEN STRIP_TAC THEN VAL_INT64_TAC `i:num` THEN
+      GEN_REWRITE_TAC (RATOR_CONV o RATOR_CONV o LAND_CONV o ONCE_DEPTH_CONV)
+       [BIGNUM_FROM_MEMORY_OFFSET_EQ_HIGHDIGITS] THEN
+      ASM_REWRITE_TAC[SUB_EQ_0; GSYM NOT_LT] THEN
+      REWRITE_TAC[ARITH_RULE `k - i - 1 = k - (i + 1)`] THEN
+      REWRITE_TAC[BIGNUM_FROM_MEMORY_STEP] THEN
+      ARM_SIM'_TAC BIGNUM_COPY_EXEC (1--3) THEN
+      REWRITE_TAC[GSYM ADD1; ENUMERATEL; GSYM APPEND_ASSOC; APPEND] THEN
+      ASM_REWRITE_TAC[ADD1; GSYM WORD_ADD; VAL_WORD_BIGDIGIT] THEN
+      REWRITE_TAC[LOWDIGITS_CLAUSES] THEN ARITH_TAC;
+      X_GEN_TAC `i:num` THEN STRIP_TAC THEN VAL_INT64_TAC `i:num` THEN
+      ARM_SIM'_TAC BIGNUM_COPY_EXEC (1--2);
+      ARM_SIM'_TAC BIGNUM_COPY_EXEC (1--2) THEN
+      ASM_SIMP_TAC[LOWDIGITS_SELF];
+      REWRITE_TAC[NSUM_CONST_NUMSEG] THEN ASM_ARITH_TAC];
+    ALL_TAC] THEN
+
+  (*** Degenerate case of no padding (initial k <= n) ***)
+
+  FIRST_X_ASSUM(DISJ_CASES_THEN2 SUBST_ALL_TAC ASSUME_TAC o
+    MATCH_MP (ARITH_RULE `n:num <= k ==> n = k \/ n < k`)) THENL
+   [SUBST1_TAC (ARITH_RULE `2 + 4 * (k - k) = 2`) THEN
+    ARM_SIM'_TAC BIGNUM_COPY_EXEC (1--2) THEN
+    REWRITE_TAC [ENUMERATEL; APPEND];
+    ALL_TAC] THEN
+
+  FIRST_ASSUM(MP_TAC o MATCH_MP (ONCE_REWRITE_RULE[IMP_CONJ]
+      NONOVERLAPPING_IMP_SMALL_2)) THEN
+    ANTS_TAC THENL [SIMPLE_ARITH_TAC; DISCH_TAC] THEN
+
+  (*** Main padding loop ***)
+
+  SUBGOAL_THEN `~(k:num <= n)` ASSUME_TAC THENL
+   [ASM_REWRITE_TAC[NOT_LE]; ALL_TAC] THEN
+
+  (*** Simplifying events ***)
+  
+  REWRITE_TAC [GSYM APPEND_ASSOC] THEN
+  SPEC_TAC(`APPEND (ENUMERATEL n (\i. [EventStore (word_add z (word (8 * i))); EventLoad (word_add x (word (8 * i)))])) es`,`es:armevent list`) THEN
+  GEN_TAC THEN
+  
+  ENSURES_N_WHILE_AUP_TAC `n:num` `k:num` `pc + 0x2c` `pc + 0x34`
+   `\i s. read X0 s = word k /\
+          read X1 s = z /\
+          read X4 s = word i /\
+          bignum_from_memory(z,i) s = a /\
+          read events s = APPEND (ENUMERATEL (i - n) (\j. [EventStore (word_add z (word (8 * (n + j))))])) es`
+   `(\i:num. 2)` `2` `2` `2` THEN
+  ASM_REWRITE_TAC[] THEN REPEAT CONJ_TAC THENL
+   [REWRITE_TAC[ARITH_RULE `n - n = 0`; ENUMERATEL; APPEND] THEN
+    ARM_SIM'_TAC BIGNUM_COPY_EXEC (1--2);
+    X_GEN_TAC `i:num` THEN STRIP_TAC THEN VAL_INT64_TAC `i:num` THEN
+    REWRITE_TAC[BIGNUM_FROM_MEMORY_STEP] THEN
+    ARM_SIM'_TAC BIGNUM_COPY_EXEC (1--2) THEN
+    SUBGOAL_THEN `(i + 1) - n = i - n + 1` SUBST1_TAC THENL [ASM_ARITH_TAC; ALL_TAC] THEN
+    SUBGOAL_THEN `n + i - n = i` ASSUME_TAC THENL [ASM_ARITH_TAC; ALL_TAC] THEN
+    ASM_REWRITE_TAC[GSYM ADD1; ENUMERATEL; GSYM APPEND_ASSOC; APPEND] THEN
+    REWRITE_TAC[ADD1; VAL_WORD_0; MULT_CLAUSES; ADD_CLAUSES; WORD_ADD];
+    X_GEN_TAC `i:num` THEN STRIP_TAC THEN VAL_INT64_TAC `i:num` THEN
+    ARM_SIM'_TAC BIGNUM_COPY_EXEC (1--2);
+    ARM_SIM'_TAC BIGNUM_COPY_EXEC (1--2);
+    REWRITE_TAC[NSUM_CONST_NUMSEG] THEN ASM_ARITH_TAC]);;
+
+let BIGNUM_COPY_CORRECT' = prove
+ (`!k z n x a pc.
+ nonoverlapping (word pc,0x40) (z,8 * val k) /\
+ (x = z \/ nonoverlapping (x,8 * MIN (val n) (val k)) (z,8 * val k))
+ ==> ensures_n arm
+       (\s. aligned_bytes_loaded s (word pc) bignum_copy_mc /\
+            read PC s = word pc /\
+            C_ARGUMENTS [k; z; n; x] s /\
+            bignum_from_memory (x,val n) s = a)
+       (\s. read PC s = word (pc + 0x3c) /\
+            bignum_from_memory (z,val k) s = lowdigits a (val k))
+       (MAYCHANGE [PC; X2; X4; X5] ,, MAYCHANGE SOME_FLAGS ,,
+        MAYCHANGE [memory :> bignum(z,val k)] ,,
+        MAYCHANGE [events])
+       (\s. 4 * val k + MIN (val n) (val k) + 6)`,
+  DROP_EVENTS_COND_TAC BIGNUM_COPY_ALL);;
+
+let BIGNUM_COPY_SUBROUTINE_CORRECT' = prove
+ (`!k z n x a pc returnaddress.
+     nonoverlapping (word pc,0x40) (z,8 * val k) /\
+     (x = z \/ nonoverlapping(x,8 * MIN (val n) (val k)) (z,8 * val k))
+     ==> ensures_n arm
+           (\s. aligned_bytes_loaded s (word pc) bignum_copy_mc  /\
+                read PC s = word pc /\
+                read X30 s = returnaddress /\
+                C_ARGUMENTS [k; z; n; x] s /\
+                bignum_from_memory (x,val n) s = a)
+           (\s. read PC s = returnaddress /\
+                bignum_from_memory (z,val k) s =  lowdigits a (val k))
+           (MAYCHANGE_REGS_AND_FLAGS_PERMITTED_BY_ABI ,,
+            MAYCHANGE [memory :> bignum(z,val k)] ,,
+            MAYCHANGE [events])
+           (\s. 4 * val k + MIN (val n) (val k) + 7)`,
+  REWRITE_TAC[ARITH_RULE `a + b + 7 = (a + b + 6) + 1`] THEN
+  ARM_ADD_RETURN_NOSTACK'_TAC BIGNUM_COPY_EXEC BIGNUM_COPY_CORRECT');;
+
 let BIGNUM_COPY_CORRECT = prove
  (`!k z n x a pc.
      nonoverlapping (word pc,0x40) (z,8 * val k) /\
@@ -50,118 +254,10 @@ let BIGNUM_COPY_CORRECT = prove
                 bignum_from_memory (x,val n) s = a)
            (\s. read PC s = word (pc + 0x3c) /\
                 bignum_from_memory (z,val k) s = lowdigits a (val k))
-          (MAYCHANGE [PC; X2; X4; X5] ,, MAYCHANGE SOME_FLAGS ,,
-           MAYCHANGE [memory :> bignum(z,val k)])`,
-  REWRITE_TAC[NONOVERLAPPING_CLAUSES] THEN
-  REWRITE_TAC[C_ARGUMENTS; C_RETURN; SOME_FLAGS; fst BIGNUM_COPY_EXEC] THEN
-  W64_GEN_TAC `k:num` THEN X_GEN_TAC `z:int64` THEN
-  W64_GEN_TAC `n:num` THEN X_GEN_TAC `x:int64` THEN
-  MAP_EVERY X_GEN_TAC [`a:num`; `pc:num`] THEN
-  DISCH_THEN(REPEAT_TCL CONJUNCTS_THEN ASSUME_TAC) THEN
-
-  (*** Simulate the initial computation of min(n,k) and then
-   *** recast the problem with n' = min(n,k) so we can assume
-   *** hereafter that n <= k. This makes life a bit easier since
-   *** otherwise n can actually be any number < 2^64 without
-   *** violating the preconditions.
-   ***)
-
-  ENSURES_SEQUENCE_TAC `pc + 0xc`
-   `\s. read X0 s = word k /\
-        read X1 s = z /\
-        read X2 s = word(MIN n k) /\
-        read X3 s = x /\
-        read X4 s = word 0 /\
-        bignum_from_memory (x,MIN n k) s = lowdigits a k` THEN
-  CONJ_TAC THENL
-   [REWRITE_TAC[GSYM LOWDIGITS_BIGNUM_FROM_MEMORY] THEN
-    ARM_SIM_TAC BIGNUM_COPY_EXEC (1--3) THEN
-    REWRITE_TAC[ARITH_RULE `MIN n k = if k < n then k else n`] THEN
-    MESON_TAC[];
-    REPEAT(FIRST_X_ASSUM(MP_TAC o check (vfree_in `k:num` o concl))) THEN
-    POP_ASSUM_LIST(K ALL_TAC) THEN MP_TAC(ARITH_RULE `MIN n k <= k`) THEN
-    SPEC_TAC(`lowdigits a k`,`a:num`) THEN SPEC_TAC(`MIN n k`,`n:num`) THEN
-    REPEAT GEN_TAC THEN REPEAT DISCH_TAC THEN
-    VAL_INT64_TAC `n:num` THEN BIGNUM_RANGE_TAC "n" "a"] THEN
-
-  (*** Break at the start of the padding stage ***)
-
-  ENSURES_SEQUENCE_TAC `pc + 0x24`
-   `\s. read X0 s = word k /\
-        read X1 s = z /\
-        read X4 s = word n /\
-        bignum_from_memory(z,n) s = a` THEN
-  CONJ_TAC THENL
-   [ASM_CASES_TAC `n = 0` THENL
-     [ASM_REWRITE_TAC[BIGNUM_FROM_MEMORY_TRIVIAL] THEN
-      REWRITE_TAC[MESON[] `0 = a <=> a = 0`] THEN
-      ARM_SIM_TAC BIGNUM_COPY_EXEC [1];
-      ALL_TAC] THEN
-
-    FIRST_ASSUM(MP_TAC o MATCH_MP (ONCE_REWRITE_RULE[IMP_CONJ]
-      NONOVERLAPPING_IMP_SMALL_2)) THEN
-    ANTS_TAC THENL [SIMPLE_ARITH_TAC; DISCH_TAC] THEN
-
-    (*** The main copying loop, in the case when n is nonzero ***)
-
-    ENSURES_WHILE_UP_TAC `n:num` `pc + 0x10` `pc + 0x1c`
-     `\i s. read X0 s = word k /\
-            read X1 s = z /\
-            read X2 s = word n /\
-            read X3 s = x /\
-            read X4 s = word i /\
-            bignum_from_memory(z,i) s = lowdigits a i /\
-            bignum_from_memory(word_add x (word(8 * i)),n - i) s =
-            highdigits a i` THEN
-    ASM_REWRITE_TAC[] THEN REPEAT CONJ_TAC THENL
-     [ARM_SIM_TAC BIGNUM_COPY_EXEC [1]  THEN
-      REWRITE_TAC[SUB_0; GSYM BIGNUM_FROM_MEMORY_BYTES; HIGHDIGITS_0] THEN
-      REWRITE_TAC[BIGNUM_FROM_MEMORY_TRIVIAL; MULT_CLAUSES; WORD_ADD_0] THEN
-      ASM_REWRITE_TAC[BIGNUM_FROM_MEMORY_BYTES; LOWDIGITS_0];
-      X_GEN_TAC `i:num` THEN STRIP_TAC THEN VAL_INT64_TAC `i:num` THEN
-      GEN_REWRITE_TAC (RATOR_CONV o LAND_CONV o ONCE_DEPTH_CONV)
-       [BIGNUM_FROM_MEMORY_OFFSET_EQ_HIGHDIGITS] THEN
-      ASM_REWRITE_TAC[SUB_EQ_0; GSYM NOT_LT] THEN
-      REWRITE_TAC[ARITH_RULE `k - i - 1 = k - (i + 1)`] THEN
-      REWRITE_TAC[BIGNUM_FROM_MEMORY_STEP] THEN
-      ARM_SIM_TAC BIGNUM_COPY_EXEC (1--3) THEN
-      ASM_REWRITE_TAC[GSYM WORD_ADD; VAL_WORD_BIGDIGIT] THEN
-      REWRITE_TAC[LOWDIGITS_CLAUSES] THEN ARITH_TAC;
-      X_GEN_TAC `i:num` THEN STRIP_TAC THEN VAL_INT64_TAC `i:num` THEN
-      ARM_SIM_TAC BIGNUM_COPY_EXEC (1--2);
-      ARM_SIM_TAC BIGNUM_COPY_EXEC (1--2) THEN
-      ASM_SIMP_TAC[LOWDIGITS_SELF]];
-    ALL_TAC] THEN
-
-  (*** Degenerate case of no padding (initial k <= n) ***)
-
-  FIRST_X_ASSUM(DISJ_CASES_THEN2 SUBST_ALL_TAC ASSUME_TAC o
-    MATCH_MP (ARITH_RULE `n:num <= k ==> n = k \/ n < k`))
-  THENL [ARM_SIM_TAC BIGNUM_COPY_EXEC (1--2); ALL_TAC] THEN
-
-  FIRST_ASSUM(MP_TAC o MATCH_MP (ONCE_REWRITE_RULE[IMP_CONJ]
-      NONOVERLAPPING_IMP_SMALL_2)) THEN
-    ANTS_TAC THENL [SIMPLE_ARITH_TAC; DISCH_TAC] THEN
-
-  (*** Main padding loop ***)
-
-  SUBGOAL_THEN `~(k:num <= n)` ASSUME_TAC THENL
-   [ASM_REWRITE_TAC[NOT_LE]; ALL_TAC] THEN
-
-  ENSURES_WHILE_AUP_TAC `n:num` `k:num` `pc + 0x2c` `pc + 0x34`
-   `\i s. read X0 s = word k /\
-          read X1 s = z /\
-          read X4 s = word i /\
-          bignum_from_memory(z,i) s = a` THEN
-  ASM_REWRITE_TAC[] THEN REPEAT CONJ_TAC THENL
-   [ARM_SIM_TAC BIGNUM_COPY_EXEC (1--2);
-    X_GEN_TAC `i:num` THEN STRIP_TAC THEN VAL_INT64_TAC `i:num` THEN
-    REWRITE_TAC[BIGNUM_FROM_MEMORY_STEP] THEN
-    ARM_SIM_TAC BIGNUM_COPY_EXEC (1--2) THEN
-    REWRITE_TAC[VAL_WORD_0; MULT_CLAUSES; ADD_CLAUSES; WORD_ADD];
-    X_GEN_TAC `i:num` THEN STRIP_TAC THEN VAL_INT64_TAC `i:num` THEN
-    ARM_SIM_TAC BIGNUM_COPY_EXEC (1--2);
-    ARM_SIM_TAC BIGNUM_COPY_EXEC (1--2)]);;
+           (MAYCHANGE [PC; X2; X4; X5] ,, MAYCHANGE SOME_FLAGS ,,
+            MAYCHANGE [memory :> bignum(z,val k)] ,,
+            MAYCHANGE [events])`,
+  ENSURES_N_ENSURES_TAC BIGNUM_COPY_CORRECT');;
 
 let BIGNUM_COPY_SUBROUTINE_CORRECT = prove
  (`!k z n x a pc returnaddress.
@@ -175,6 +271,59 @@ let BIGNUM_COPY_SUBROUTINE_CORRECT = prove
                 bignum_from_memory (x,val n) s = a)
            (\s. read PC s = returnaddress /\
                 bignum_from_memory (z,val k) s =  lowdigits a (val k))
-          (MAYCHANGE_REGS_AND_FLAGS_PERMITTED_BY_ABI ,,
-           MAYCHANGE [memory :> bignum(z,val k)])`,
-  ARM_ADD_RETURN_NOSTACK_TAC BIGNUM_COPY_EXEC BIGNUM_COPY_CORRECT);;
+           (MAYCHANGE_REGS_AND_FLAGS_PERMITTED_BY_ABI ,,
+            MAYCHANGE [memory :> bignum(z,val k)] ,,
+            MAYCHANGE [events])`,
+  ENSURES_N_ENSURES_TAC BIGNUM_COPY_SUBROUTINE_CORRECT');;
+
+let BIGNUM_COPY_CONST_TIME = prove
+ (`?f_es. !es1 es2 k:int64 z:int64 n:int64 x:int64 a1:num a2:num pc1 pc2 es1 es2.
+    nonoverlapping (word pc1,0x40) (z,8 * val k) /\ nonoverlapping (word pc2,0x40) (z,8 * val k) /\
+    (x = z \/ nonoverlapping(x,8 * MIN (val n) (val k)) (z,8 * val k))
+    ==>
+    ensures2 arm
+      (\(s1,s2). aligned_bytes_loaded s1 (word pc1) bignum_copy_mc /\ read PC s1 = word pc1 /\
+                 aligned_bytes_loaded s2 (word pc2) bignum_copy_mc /\ read PC s2 = word pc2 /\
+                 C_ARGUMENTS [k; z; n; x] s1 /\ C_ARGUMENTS [k; z; n; x] s2 /\
+                 bignum_from_memory (x,val n) s1 = a1 /\ bignum_from_memory (x,val n) s2 = a2 /\
+                 read events s1 = es1 /\ read events s2 = es2)
+      (\(s1,s2). read PC s1 = word (pc1 + 0x3c) /\ read PC s2 = word (pc2 + 0x3c) /\
+                 bignum_from_memory (z,val k) s1 = lowdigits a1 (val k) /\ bignum_from_memory (z,val k) s2 = lowdigits a2 (val k) /\
+                 read events s1 = APPEND (f_es (val k) z (val n) x) es1 /\
+                 read events s2 = APPEND (f_es (val k) z (val n) x) es2)
+      (\(s1,s2) (s1',s2').
+        (MAYCHANGE [PC; X2; X4; X5] ,, MAYCHANGE SOME_FLAGS ,, MAYCHANGE [memory :> bignum(z,val k)] ,, MAYCHANGE [events]) s1 s1' /\
+        (MAYCHANGE [PC; X2; X4; X5] ,, MAYCHANGE SOME_FLAGS ,, MAYCHANGE [memory :> bignum(z,val k)] ,, MAYCHANGE [events]) s2 s2')
+      (\s. 4 * val k + MIN (val n) (val k) + 6)
+      (\s. 4 * val k + MIN (val n) (val k) + 6)`,
+  CHOOSE_THEN ASSUME_TAC BIGNUM_COPY_ALL THEN
+  EXISTS_TAC `f_es:num->int64->num->int64->armevent list` THEN
+  REPEAT GEN_TAC THEN REPEAT DISCH_TAC THEN
+  PURE_REWRITE_TAC
+    [MESON[] `!s1 s2.
+       (aligned_bytes_loaded s1 (word pc1) bignum_copy_mc /\ read PC s1 = word pc1 /\
+        aligned_bytes_loaded s2 (word pc2) bignum_copy_mc /\ read PC s2 = word pc2 /\
+        C_ARGUMENTS [k; z; n; x] s1 /\ C_ARGUMENTS [k; z; n; x] s2 /\
+        bignum_from_memory (x,val n) s1 = a1 /\ bignum_from_memory (x,val n) s2 = a2 /\
+        read events s1 = es1 /\ read events s2 = es2)
+       =
+       ((\s1. aligned_bytes_loaded s1 (word pc1) bignum_copy_mc /\ read PC s1 = word pc1 /\
+              C_ARGUMENTS [k; z; n; x] s1 /\ bignum_from_memory (x,val n) s1 = a1 /\ read events s1 = es1) s1 /\
+        (\s2. aligned_bytes_loaded s2 (word pc2) bignum_copy_mc /\ read PC s2 = word pc2 /\
+              C_ARGUMENTS [k; z; n; x] s2 /\ bignum_from_memory (x,val n) s2 = a2 /\ read events s2 = es2) s2)`;
+     MESON[] `!s1 s2.
+       (read PC s1 = word (pc1 + 0x3c) /\ read PC s2 = word (pc2 + 0x3c) /\
+        bignum_from_memory (z,val k) s1 = lowdigits a1 (val k) /\ bignum_from_memory (z,val k) s2 = lowdigits a2 (val k) /\
+        read events s1 = APPEND (f_es (val k) z (val n) x) es1 /\ read events s2 = APPEND (f_es (val k) z (val n) x) es2)
+       =
+       ((\s1. read PC s1 = word (pc1 + 0x3c) /\ bignum_from_memory (z,val k) s1 = lowdigits a1 (val k) /\
+              read events s1 = APPEND (f_es (val k) z (val n) x) es1) s1 /\
+        (\s2. read PC s2 = word (pc2 + 0x3c) /\ bignum_from_memory (z,val k) s2 = lowdigits a2 (val k) /\
+              read events s2 = APPEND (f_es (val k) z (val n) x) es2) s2)`] THEN
+  MATCH_MP_TAC COMBINE_ENSURES_N_ENSURES2 THEN
+  SUBGOAL_THEN `!z:int64 k:int64. (\s2 s2'.
+    (MAYCHANGE [PC; X2; X4; X5] ,, MAYCHANGE SOME_FLAGS ,, MAYCHANGE [memory :> bignum (z,val k)] ,, MAYCHANGE [events]) s2 s2')
+    =
+    (MAYCHANGE [PC; X2; X4; X5] ,, MAYCHANGE SOME_FLAGS ,, MAYCHANGE [memory :> bignum (z,val k)] ,, MAYCHANGE [events])`
+    ASSUME_TAC THENL [REPEAT GEN_TAC THEN SIMP_TAC[FUN_EQ_THM]; ALL_TAC] THEN
+  ASM_SIMP_TAC[]);;
