arm/proofs/bignum_copy_2.ml
@@ -1,0 +1,276 @@
+(*
+ * Copyright Amazon.com, Inc. or its affiliates. All Rights Reserved.
+ * SPDX-License-Identifier: Apache-2.0 OR ISC OR MIT-0
+ *)
+
+(* ========================================================================= *)
+(* Copying (with truncation or extension) bignums                            *)
+(* ========================================================================= *)
+
+needs "arm/proofs/equiv.ml";;
+
+(**** print_literal_from_elf "arm/generic/bignum_copy.o";;
+ ****)
+
+let ITE_SAME = prove(`(if b then x else x) = x`, MESON_TAC []);;
+
+let bignum_copy_mc = define_assert_from_elf "bignum_copy_mc" "arm/generic/bignum_copy.o" [
+  0xeb02001f;       (* arm_CMP X0 X2 *)
+  0x9a823002;       (* arm_CSEL X2 X0 X2 Condition_CC *)
+  0xd2800004;       (* arm_MOV X4 (rvalue (word 0)) *)
+  0xb40000c2;       (* arm_CBZ X2 (word 24) *)
+  0xf8647865;       (* arm_LDR X5 X3 (Shiftreg_Offset X4 3) *)
+  0xf8247825;       (* arm_STR X5 X1 (Shiftreg_Offset X4 3) *)
+  0x91000484;       (* arm_ADD X4 X4 (rvalue (word 1)) *)
+  0xeb02009f;       (* arm_CMP X4 X2 *)
+  0x54ffff83;       (* arm_BCC (word 2097136) *)
+  0xeb00009f;       (* arm_CMP X4 X0 *)
+  0x540000a2;       (* arm_BCS (word 20) *)
+  0xf824783f;       (* arm_STR XZR X1 (Shiftreg_Offset X4 3) *)
+  0x91000484;       (* arm_ADD X4 X4 (rvalue (word 1)) *)
+  0xeb00009f;       (* arm_CMP X4 X0 *)
+  0x54ffffa3;       (* arm_BCC (word 2097140) *)
+  0xd65f03c0        (* arm_RET X30 *)
+];;
+
+let COPY_EXEC = ARM_MK_EXEC_RULE bignum_copy_mc;;
+
+(* Symbolic execution of the two programs, going through n small steps. *)
+let straight_line_tac (n:int):tactic =
+  ENSURES2_INIT_TAC "s0" "s0'" THEN
+  REPEAT_N (if n == 0 then 0 else 1) (
+    MAP_EVERY ASSUME_STEPS_ID ["s0";"s0'"] THEN
+    ASSUME_TAC(ISPEC (mk_var("s0'",`:armstate`)) MAYCHANGE_STARTER) THEN
+    ABBREV_TAC `es = read events s0'` THEN
+    ARM_STUTTER_LEFT_TAC COPY_EXEC (1--n) THEN
+    ARM_STUTTER_RIGHT_TAC COPY_EXEC (1--n) "'") THEN
+  REPEAT_N 2 ENSURES_FINAL_STATE'_TAC THEN
+  ASM_REWRITE_TAC[WORD_ADD];;
+
+let INIT_CONST_TIME = prove(
+  `!pc1 pc2 k z n x.
+    k < 2 EXP 64 /\ n < 2 EXP 64
+    ==> ensures2 arm
+      (\(s1,s2). aligned_bytes_loaded s1 (word pc1) bignum_copy_mc /\ read PC s1 = word pc1 /\
+                 aligned_bytes_loaded s2 (word pc2) bignum_copy_mc /\ read PC s2 = word pc2 /\
+                 C_ARGUMENTS [word k; z; word n; x] s1 /\
+                 C_ARGUMENTS [word k; z; word n; x] s2 /\
+                 read events s1 = read events s2)
+      (\(s1,s2). aligned_bytes_loaded s1 (word pc1) bignum_copy_mc /\
+                 (~(0 = MIN k n) /\ read PC s1 = word (pc1 + 0x10) \/ 0 = MIN k n /\ read PC s1 = word (pc1 + 0x24)) /\
+                 aligned_bytes_loaded s2 (word pc2) bignum_copy_mc /\
+                 (~(0 = MIN k n) /\ read PC s2 = word (pc2 + 0x10) \/ 0 = MIN k n /\ read PC s2 = word (pc2 + 0x24)) /\
+                 C_ARGUMENTS [word k; z; word (MIN k n); x; word 0] s1 /\
+                 C_ARGUMENTS [word k; z; word (MIN k n); x; word 0] s2 /\
+                 read events s1 = read events s2)
+      (\s s'. T)
+      (\s. 4)
+      (\s. 4)`,
+  let finish =
+    IMP_REWRITE_TAC [VAL_WORD; DIMINDEX_64; MOD_LT; ITE_SAME] THEN
+    COND_CASES_TAC THENL replicate (
+    ASM_REWRITE_TAC []) 2 in
+  IMP_REWRITE_TAC [C_ARGUMENTS; MIN] THEN
+  REPEAT STRIP_TAC THEN
+  straight_line_tac 4 THEN
+  DISJ_CASES_TAC (SPEC `k < n` EXCLUDED_MIDDLE) THENL [
+    ASSUME_TAC (ARITH_RULE `k < n ==> k <= n`) THEN
+    finish;
+    DISJ_CASES_TAC (SPEC `k:num = n` EXCLUDED_MIDDLE) THENL [
+      finish;
+      ASSUME_TAC (ARITH_RULE `~(k < n) /\ ~(k = n) ==> ~(k <= n)`) THEN
+      finish]]);;
+
+let COPYLOOP_CONST_TIME = prove(
+  `!pc1 pc2 k z n x.
+    k < 2 EXP 64 /\ n < 2 EXP 64 /\ ~(0 = MIN k n) /\
+    nonoverlapping (word pc1, 0x40) (z, 8 * k) /\ nonoverlapping (word pc2, 0x40) (z, 8 * k)
+    ==> ensures2 arm
+      (\(s1,s2). aligned_bytes_loaded s1 (word pc1) bignum_copy_mc /\ read PC s1 = word (pc1 + 0x10) /\
+                 aligned_bytes_loaded s2 (word pc2) bignum_copy_mc /\ read PC s2 = word (pc2 + 0x10) /\
+                 C_ARGUMENTS [word k; z; word (MIN k n); x; word 0] s1 /\
+                 C_ARGUMENTS [word k; z; word (MIN k n); x; word 0] s2 /\
+                 read events s1 = read events s2)
+      (\(s1,s2). aligned_bytes_loaded s1 (word pc1) bignum_copy_mc /\ read PC s1 = word (pc1 + 0x24) /\
+                 aligned_bytes_loaded s2 (word pc2) bignum_copy_mc /\ read PC s2 = word (pc2 + 0x24) /\
+                 C_ARGUMENTS [word k; z; word (MIN k n); x; word (MIN k n)] s1 /\
+                 C_ARGUMENTS [word k; z; word (MIN k n); x; word (MIN k n)] s2 /\
+                 read events s1 = read events s2)
+      (\s s'. T)
+      (\s. 5 * MIN k n)
+      (\s. 5 * MIN k n)`,
+  REWRITE_TAC [C_ARGUMENTS; NONOVERLAPPING_CLAUSES] THEN
+  REPEAT STRIP_TAC THEN
+  ENSURES2_WHILE_PAUP_TAC `0:num` `MIN k n` `pc1 + 0x10` `pc1 + 0x20` `pc2 + 0x10` `pc2 + 0x20`
+  `\i s1 s2.
+      (read X0 s1 = word k /\ read X1 s1 = z /\ read X2 s1 = word (MIN k n) /\ read X3 s1 = x /\ read X4 s1 = word i) /\
+      (read X0 s2 = word k /\ read X1 s2 = z /\ read X2 s2 = word (MIN k n) /\ read X3 s2 = x /\ read X4 s2 = word i) /\
+      read events s1 = read events s2`
+  `\(i:num) s. read CF s <=> MIN k n <= i`
+  `\(i:num) s. read CF s <=> MIN k n <= i`
+  `\(i:num). 4`
+  `\(i:num). 4`
+  `0` `0` `1` `1` THEN
+  REPEAT CONJ_TAC THENL [
+    (* # loop itrs > 0 *)
+    ASM_ARITH_TAC;
+    (* entrace -> loop header *)
+    straight_line_tac 0;
+    (* the main loop! *)
+    REPEAT STRIP_TAC THEN
+    SUBGOAL_THEN `i < k` ASSUME_TAC THENL [ASM_ARITH_TAC; ALL_TAC] THEN
+    SUBGOAL_THEN `i < 2 EXP 64` ASSUME_TAC THENL [ASM_ARITH_TAC; ALL_TAC] THEN
+    SUBGOAL_THEN `val (word i:64 word) < k` ASSUME_TAC THENL [IMP_REWRITE_TAC [VAL_WORD; DIMINDEX_64; MOD_LT]; ALL_TAC] THEN
+    straight_line_tac 4 THEN
+    SUBGOAL_THEN `k < 2 EXP 64 /\ n < 2 EXP 64 ==> MIN k n < 2 EXP 64` ASSUME_TAC THENL [ARITH_TAC; ALL_TAC] THEN
+    REWRITE_TAC[VAL_WORD_SUB_EQ_0; GSYM WORD_ADD; VAL_WORD; DIMINDEX_64] THEN
+    IMP_REWRITE_TAC [MOD_LT; ARITH_RULE `i < MIN k n /\ MIN k n < 2 EXP 64 ==> i + 1 < 2 EXP 64`];
+    (* backedge *)
+    REPEAT STRIP_TAC THEN
+    straight_line_tac 1;
+    (* postcond to ret *)
+    ALL_TAC;
+    (* counter 1 *)
+    REWRITE_TAC[NSUM_CONST_NUMSEG] THEN ASM_ARITH_TAC;
+    (* counter 2 *)
+    REWRITE_TAC[NSUM_CONST_NUMSEG] THEN ASM_ARITH_TAC] THEN
+  straight_line_tac 1);;
+
+let PADDING_CONST_TIME = prove(
+  `!pc1 pc2 k z n x.
+    k < 2 EXP 64 /\ n < 2 EXP 64
+    ==> ensures2 arm
+      (\(s1,s2). aligned_bytes_loaded s1 (word pc1) bignum_copy_mc /\ read PC s1 = word (pc1 + 0x24) /\
+                 aligned_bytes_loaded s2 (word pc2) bignum_copy_mc /\ read PC s2 = word (pc2 + 0x24) /\
+                 C_ARGUMENTS [word k; z; word (MIN k n); x; word (MIN k n)] s1 /\
+                 C_ARGUMENTS [word k; z; word (MIN k n); x; word (MIN k n)] s2 /\
+                 read events s1 = read events s2)
+      (\(s1,s2). aligned_bytes_loaded s1 (word pc1) bignum_copy_mc /\
+                 (~(k <= MIN k n) /\ read PC s1 = word (pc1 + 0x2c) \/ k <= MIN k n /\ read PC s1 = word (pc1 + 0x3c)) /\
+                 aligned_bytes_loaded s2 (word pc2) bignum_copy_mc /\
+                 (~(k <= MIN k n) /\ read PC s2 = word (pc2 + 0x2c) \/ k <= MIN k n /\ read PC s2 = word (pc2 + 0x3c)) /\
+                 C_ARGUMENTS [word k; z; word (MIN k n); x; word (MIN k n)] s1 /\
+                 C_ARGUMENTS [word k; z; word (MIN k n); x; word (MIN k n)] s2 /\
+                 read events s1 = read events s2)
+      (\s s'. T)
+      (\s. 2)
+      (\s. 2)`,
+  REWRITE_TAC [C_ARGUMENTS] THEN
+  REPEAT STRIP_TAC THEN
+  SUBGOAL_THEN `MIN k n < 2 EXP 64` ASSUME_TAC THENL [ASM_ARITH_TAC; ALL_TAC] THEN
+  straight_line_tac 2 THEN
+  DISJ_CASES_TAC (SPEC `k <= MIN k n` EXCLUDED_MIDDLE) THENL [
+    IMP_REWRITE_TAC [VAL_WORD; DIMINDEX_64; MOD_LT];
+    IMP_REWRITE_TAC [VAL_WORD; DIMINDEX_64; MOD_LT] THEN
+    ASM_REWRITE_TAC [GSYM NOT_LE]]);;
+
+let PADLOOP_CONST_TIME = prove(
+  `!pc1 pc2 k z n x.
+    k < 2 EXP 64 /\ n < 2 EXP 64 /\ ~(k <= MIN k n) /\
+    nonoverlapping (word pc1, 0x40) (z, 8 * k) /\ nonoverlapping (word pc2, 0x40) (z, 8 * k)
+    ==> ensures2 arm
+      (\(s1,s2). aligned_bytes_loaded s1 (word pc1) bignum_copy_mc /\ read PC s1 = word (pc1 + 0x2c) /\
+                 aligned_bytes_loaded s2 (word pc2) bignum_copy_mc /\ read PC s2 = word (pc2 + 0x2c) /\
+                 C_ARGUMENTS [word k; z; word (MIN k n); x; word (MIN k n)] s1 /\
+                 C_ARGUMENTS [word k; z; word (MIN k n); x; word (MIN k n)] s2 /\
+                 read events s1 = read events s2)
+      (\(s1,s2). aligned_bytes_loaded s1 (word pc1) bignum_copy_mc /\ read PC s1 = word (pc1 + 0x3c) /\
+                 aligned_bytes_loaded s2 (word pc2) bignum_copy_mc /\ read PC s2 = word (pc2 + 0x3c) /\
+                 C_ARGUMENTS [word k; z; word (MIN k n); x; word k] s1 /\
+                 C_ARGUMENTS [word k; z; word (MIN k n); x; word k] s2 /\
+                 read events s1 = read events s2)
+      (\s s'. T)
+      (\s. 4 * (k - (MIN k n)))
+      (\s. 4 * (k - (MIN k n)))`,
+  REWRITE_TAC [C_ARGUMENTS; NONOVERLAPPING_CLAUSES] THEN
+  REPEAT STRIP_TAC THEN
+  ENSURES2_WHILE_PAUP_TAC `(MIN k n):num` `k:num` `pc1 + 0x2c` `pc1 + 0x38` `pc2 + 0x2c` `pc2 + 0x38`
+  `\i s1 s2.
+      read X0 s1 = word k /\ read X1 s1 = z /\ read X2 s1 = word (MIN k n) /\ read X3 s1 = x /\ read X4 s1 = word i /\
+      read X0 s2 = word k /\ read X1 s2 = z /\ read X2 s2 = word (MIN k n) /\ read X3 s2 = x /\ read X4 s2 = word i /\
+      read events s1 = read events s2`
+  `\(i:num) s. read CF s <=> k <= i`
+  `\(i:num) s. read CF s <=> k <= i`
+  `\(i:num). 3`
+  `\(i:num). 3`
+  `0` `0` `1` `1` THEN
+  REPEAT CONJ_TAC THENL [
+    (* # loop itrs > 0 *)
+    ASM_ARITH_TAC;
+    (* entrace -> loop header *)
+    straight_line_tac 0;
+    (* the main loop! *)
+    REPEAT STRIP_TAC THEN
+    SUBGOAL_THEN `i < 2 EXP 64` ASSUME_TAC THENL [ASM_ARITH_TAC; ALL_TAC] THEN
+    SUBGOAL_THEN `val (word i:64 word) < k` ASSUME_TAC THENL [IMP_REWRITE_TAC [VAL_WORD; DIMINDEX_64; MOD_LT]; ALL_TAC] THEN
+    straight_line_tac 3 THEN
+    REWRITE_TAC [VAL_WORD_SUB_EQ_0; GSYM WORD_ADD; VAL_WORD; DIMINDEX_64] THEN
+    IMP_REWRITE_TAC [MOD_LT; ARITH_RULE `i < n /\ n < 2 EXP 64 ==> i + 1 < 2 EXP 64`];
+    (* backedge *)
+    REPEAT STRIP_TAC THEN
+    straight_line_tac 1;
+    (* postcond to ret *)
+    straight_line_tac 1;
+    (* counter 1 *)
+    REWRITE_TAC [NSUM_CONST_NUMSEG] THEN ASM_ARITH_TAC;
+    (* counter 2 *)
+    REWRITE_TAC [NSUM_CONST_NUMSEG] THEN ASM_ARITH_TAC]);;
+
+let COPY_CONST_TIME = prove(
+  `!pc1 pc2 k z n x.
+    k < 2 EXP 64 /\ n < 2 EXP 64 /\
+    nonoverlapping (word pc1, 0x40) (z, 8 * k) /\ nonoverlapping (word pc2, 0x40) (z, 8 * k)
+    ==> ensures2 arm
+      (\(s1,s2). aligned_bytes_loaded s1 (word pc1) bignum_copy_mc /\ read PC s1 = word pc1 /\
+                 aligned_bytes_loaded s2 (word pc2) bignum_copy_mc /\ read PC s2 = word pc2 /\
+                 C_ARGUMENTS [word k; z; word n; x] s1 /\
+                 C_ARGUMENTS [word k; z; word n; x] s2 /\
+                 read events s1 = read events s2)
+      (\(s1,s2). aligned_bytes_loaded s1 (word pc1) bignum_copy_mc /\ read PC s1 = word (pc1 + 0x3c) /\
+                 aligned_bytes_loaded s2 (word pc2) bignum_copy_mc /\ read PC s2 = word (pc2 + 0x3c) /\
+                 C_ARGUMENTS [word k; z; word (MIN k n); x; word k] s1 /\
+                 C_ARGUMENTS [word k; z; word (MIN k n); x; word k] s2 /\
+                 read events s1 = read events s2)
+      ((\s s'. T))
+      (\s. 4 + 5 * MIN k n + 2 + 4 * (k - (MIN k n)))
+      (\s. 4 + 5 * MIN k n + 2 + 4 * (k - (MIN k n)))`,
+  REPEAT STRIP_TAC THEN
+  ONCE_REWRITE_TAC [GSYM (INST_TYPE [`:armstate#armstate`, `:B`] COMPONENT_SINK)] THEN
+  MATCH_MP_TAC ENSURES2_TRANS THEN
+  META_EXISTS_TAC THEN
+  CONJ_TAC THENL [
+    MP_TAC (SPEC_ALL INIT_CONST_TIME) THEN
+    ASM_REWRITE_TAC [] THEN
+    DISCH_THEN (UNIFY_ACCEPT_TAC [`Q:armstate#armstate->bool`]);
+    ALL_TAC;
+  ] THEN
+  ONCE_REWRITE_TAC [GSYM (INST_TYPE [`:armstate#armstate`, `:B`] COMPONENT_SINK)] THEN
+  MATCH_MP_TAC ENSURES2_TRANS THEN
+  META_EXISTS_TAC THEN
+  CONJ_TAC THENL [
+    DISJ_CASES_TAC (SPEC `0 = MIN k n` EXCLUDED_MIDDLE) THENL [
+      REWRITE_TAC [SYM (ASSUME `0 = MIN k n`); MULT_0] THEN
+      IMP_REWRITE_TAC [ENSURES2_TRIVIAL] THEN
+      REWRITE_TAC [] THEN
+      STRIP_TAC THEN
+      DISCH_THEN (UNIFY_ACCEPT_TAC [`Q:armstate#armstate->bool`]);
+      ASM_REWRITE_TAC [] THEN
+      MP_TAC (SPEC_ALL COPYLOOP_CONST_TIME) THEN
+      ASM_REWRITE_TAC []];
+      ALL_TAC] THEN
+  ONCE_REWRITE_TAC [GSYM (INST_TYPE [`:armstate#armstate`, `:B`] COMPONENT_SINK)] THEN
+  MATCH_MP_TAC ENSURES2_TRANS THEN
+  META_EXISTS_TAC THEN
+  CONJ_TAC THENL [
+    MP_TAC (SPEC_ALL PADDING_CONST_TIME) THEN
+    ASM_REWRITE_TAC [] THEN
+    DISCH_THEN (UNIFY_ACCEPT_TAC [`Q:armstate#armstate->bool`]);
+    ALL_TAC;
+  ] THEN
+  DISJ_CASES_TAC (SPEC `k <= MIN k n` EXCLUDED_MIDDLE) THENL [
+    SUBGOAL_THEN `MIN k n = k` ASSUME_TAC THENL [ASM_ARITH_TAC; ALL_TAC] THEN
+    SUBGOAL_THEN `4 * (k - MIN k n) = 0` ASSUME_TAC THENL [ASM_ARITH_TAC; ALL_TAC] THEN
+    IMP_REWRITE_TAC [ENSURES2_TRIVIAL] THEN
+    REWRITE_TAC [];
+    ASM_REWRITE_TAC [] THEN
+    IMP_REWRITE_TAC [PADLOOP_CONST_TIME]]);;
