common/bignum_n.ml
@@ -1,0 +1,24 @@
+(* ------------------------------------------------------------------------- *)
+(* Get ranges of bignum abbreviation out of precondition.                    *)
+(* ------------------------------------------------------------------------- *)
+
+let BIGNUM_TERMRANGE'_TAC =
+  let pth = prove
+   (`!k m. m < 2 EXP (64 * k) \/ !s x. ~(bignum_from_memory (x,k) s = m)`,
+    MESON_TAC[BIGNUM_FROM_MEMORY_BOUND]) in
+  fun k m ->
+    DISJ_CASES_THEN2
+     ASSUME_TAC
+     (fun th -> REWRITE_TAC[th; ENSURES_N_TRIVIAL] THEN NO_TAC)
+     (SPECL [k; m] pth);;
+
+let BIGNUM_RANGE'_TAC =
+  let pth = prove
+   (`!k m. m < 2 EXP (64 * k) \/ !s x. ~(bignum_from_memory (x,k) s = m)`,
+    MESON_TAC[BIGNUM_FROM_MEMORY_BOUND])
+  and nty = `:num` in
+  fun k m ->
+    DISJ_CASES_THEN2
+     ASSUME_TAC
+     (fun th -> REWRITE_TAC[th; ENSURES_N_TRIVIAL] THEN NO_TAC)
+     (SPECL [mk_var(k,nty); mk_var(m,nty)] pth);;
