common/relational_n.ml
@@ -1,0 +1,800 @@
+needs "common/relational.ml";;
+needs "common/relational2.ml";;
+
+let NSUM_REFLECT' = prove(`!x n. nsum (0..n) (\i. x(n - i)) = nsum (0..n) x`,
+  REPEAT GEN_TAC THEN
+  SUBST1_TAC (SPECL [`x:num->num`; `0`; `n:num`] NSUM_REFLECT) THEN
+  REWRITE_TAC [ARITH_RULE `~(n < 0) /\ (n - 0 = n)`]);;
+
+let ENSURES_N_TRIVIAL = prove(
+  `!step q f fn. ensures_n step (\x. F) q f fn`,
+  REWRITE_TAC[ensures_n]);;
+
+let ENSURES_N_ALREADY = prove(
+  `!(step:A->A->bool) P Q C n.
+    (!s. P s ==> Q s) /\ (!s. C s s) ==> ensures_n step P Q C (\s. 0)`,
+  REWRITE_TAC[ensures_n;EVENTUALLY_N_TRIVIAL] THEN
+  REWRITE_TAC[FORALL_PAIR_THM] THEN MESON_TAC[]);;
+
+let ENSURES_N_INIT_TAC sname =
+  GEN_REWRITE_TAC I [ensures_n] THEN
+  REWRITE_TAC[] (* for general beta reduction *) THEN
+  W(fun (asl,w) ->
+      let ty = type_of(fst(dest_forall w)) in
+      let svar = mk_var(sname,ty) in
+      X_GEN_TAC svar THEN
+      DISCH_THEN(REPEAT_TCL CONJUNCTS_THEN ASSUME_TAC) THEN
+      ASSUME_TAC(ISPEC svar MAYCHANGE_STARTER));;
+
+let ENSURES_N_BIGNUM_TERMRANGE_TAC =
+  let pth = prove
+   (`!k m. m < 2 EXP (64 * k) \/ !s x. ~(bignum_from_memory (x,k) s = m)`,
+    MESON_TAC[BIGNUM_FROM_MEMORY_BOUND]) in
+  fun k m ->
+    DISJ_CASES_THEN2
+     ASSUME_TAC
+     (fun th -> REWRITE_TAC[th; ENSURES_N_TRIVIAL] THEN NO_TAC)
+     (SPECL [k; m] pth);;
+
+(* ------------------------------------------------------------------------- *)
+(* Classic precondition strengthening and postcondition weakening.           *)
+(* Implement also (essentially trivial) tactics to apply it.                 *)
+(* ------------------------------------------------------------------------- *)
+
+let ENSURES_N_PRECONDITION_THM_GEN = prove
+ (`!P P' C C' Q fn.
+        (!x. P' x ==> P x) /\
+        (!x y. C x y ==> C' x y) /\
+        ensures_n step P Q C fn
+        ==> ensures_n step P' Q C' fn`,
+  REPEAT GEN_TAC THEN REWRITE_TAC[ensures_n] THEN
+  REPEAT(DISCH_THEN(CONJUNCTS_THEN2 ASSUME_TAC MP_TAC)) THEN
+  REWRITE_TAC[ensures_n] THEN MATCH_MP_TAC MONO_FORALL THEN GEN_TAC THEN
+  MATCH_MP_TAC MONO_IMP THEN REWRITE_TAC[] THEN
+  ASM_REWRITE_TAC[] THEN
+  MATCH_MP_TAC(REWRITE_RULE[RIGHT_IMP_FORALL_THM] EVENTUALLY_N_MONO) THEN
+  ASM_SIMP_TAC[]);;
+
+let ENSURES_N_PRECONDITION_THM = prove
+ (`!P P' C Q fn.
+        (!x. P' x ==> P x) /\
+        ensures_n step P Q C fn
+        ==> ensures_n step P' Q C fn`,
+  REPEAT GEN_TAC THEN REWRITE_TAC[ensures_n] THEN
+  REPEAT(DISCH_THEN(CONJUNCTS_THEN2 ASSUME_TAC MP_TAC)) THEN
+  REWRITE_TAC[ensures_n] THEN MATCH_MP_TAC MONO_FORALL THEN GEN_TAC THEN
+  MATCH_MP_TAC MONO_IMP THEN REWRITE_TAC[] THEN
+  ASM_REWRITE_TAC[]);;
+
+let ENSURES_N_PRECONDITION_TAC p' =
+  MATCH_MP_TAC ENSURES_N_PRECONDITION_THM THEN EXISTS_TAC p';;
+
+let ENSURES_N_POSTCONDITION_THM_GEN = prove
+ (`!P C C' Q Q' fn.
+        (!x. Q x ==> Q' x) /\
+        (!x y. C x y ==> C' x y) /\
+        ensures_n step P Q C fn
+        ==> ensures_n step P Q' C' fn`,
+  REPEAT GEN_TAC THEN
+  REPEAT(DISCH_THEN(CONJUNCTS_THEN2 ASSUME_TAC MP_TAC)) THEN
+  REWRITE_TAC[ensures_n] THEN MATCH_MP_TAC MONO_FORALL THEN GEN_TAC THEN
+  MATCH_MP_TAC MONO_IMP THEN REWRITE_TAC[] THEN
+  ASM_REWRITE_TAC[] THEN
+  MATCH_MP_TAC(REWRITE_RULE[RIGHT_IMP_FORALL_THM] EVENTUALLY_N_MONO) THEN
+  ASM_SIMP_TAC[]);;
+
+let ENSURES_N_POSTCONDITION_THM = prove
+ (`!P C Q Q' fn.
+        (!x. Q x ==> Q' x) /\
+        ensures_n step P Q C fn
+        ==> ensures_n step P Q' C fn`,
+  REPEAT GEN_TAC THEN
+  REPEAT(DISCH_THEN(CONJUNCTS_THEN2 ASSUME_TAC MP_TAC)) THEN
+  REWRITE_TAC[ensures_n] THEN MATCH_MP_TAC MONO_FORALL THEN GEN_TAC THEN
+  MATCH_MP_TAC MONO_IMP THEN REWRITE_TAC[] THEN
+  ASM_REWRITE_TAC[] THEN
+  MATCH_MP_TAC(REWRITE_RULE[RIGHT_IMP_FORALL_THM] EVENTUALLY_N_MONO) THEN
+  ASM_SIMP_TAC[]);;
+
+let ENSURES_N_POSTCONDITION_TAC q' =
+  MATCH_MP_TAC ENSURES_N_POSTCONDITION_THM THEN EXISTS_TAC q';;
+
+let ENSURES_N_PREPOSTCONDITION_THM = prove
+ (`!P P' C Q Q' fn.
+        (!x. P' x ==> P x) /\ (!x. Q x ==> Q' x) /\
+        ensures_n step P Q C fn
+        ==> ensures_n step P' Q' C fn`,
+  REPEAT GEN_TAC THEN REWRITE_TAC[ensures_n] THEN
+  REPEAT(DISCH_THEN(CONJUNCTS_THEN2 ASSUME_TAC MP_TAC)) THEN
+  REWRITE_TAC[ensures_n] THEN MATCH_MP_TAC MONO_FORALL THEN GEN_TAC THEN
+  MATCH_MP_TAC MONO_IMP THEN REWRITE_TAC[] THEN
+  ASM_REWRITE_TAC[] THEN
+  MATCH_MP_TAC(REWRITE_RULE[RIGHT_IMP_FORALL_THM] EVENTUALLY_N_MONO) THEN
+  ASM_SIMP_TAC[]);;
+
+(* ------------------------------------------------------------------------- *)
+(* The analogous monotonicity result for the frame.                          *)
+(* ------------------------------------------------------------------------- *)
+
+let ENSURES_N_FRAME_MONO = prove
+ (`!P Q C C' fn.
+        (!x y. C x y ==> C' x y) /\
+        ensures_n step P Q C fn
+        ==> ensures_n step P Q C' fn`,
+   REPEAT GEN_TAC THEN
+   REPEAT(DISCH_THEN(CONJUNCTS_THEN2 ASSUME_TAC MP_TAC)) THEN
+   REWRITE_TAC[ensures_n] THEN MATCH_MP_TAC MONO_FORALL THEN GEN_TAC THEN
+   MATCH_MP_TAC MONO_IMP THEN REWRITE_TAC[] THEN
+   ASM_REWRITE_TAC[] THEN
+   MATCH_MP_TAC(REWRITE_RULE[RIGHT_IMP_FORALL_THM] EVENTUALLY_N_MONO) THEN
+   ASM_SIMP_TAC[]);;
+ 
+let ENSURES_N_FRAME_SUBSUMED = prove
+ (`!P Q C C' fn.
+        C subsumed C' /\
+        ensures_n step P Q C fn
+        ==> ensures_n step P Q C' fn`,
+   REWRITE_TAC[subsumed; ENSURES_N_FRAME_MONO]);;
+
+(* ------------------------------------------------------------------------- *)
+(* Classic Hoare sequencing / Transitivity rule.                             *)
+(* ------------------------------------------------------------------------- *)
+
+let ENSURES_N_TRANS = prove(
+  `!step (P:S->bool) (Q:S->bool) (R:S->bool) C1 C2 n1 n2.
+    ensures_n step P Q C1 (\s. n1) /\ ensures_n step Q R C2 (\s. n2)
+    ==> ensures_n step P R (C1 ,, C2) (\s. n1 + n2)`,
+  REWRITE_TAC [ensures_n; eventually_n] THEN
+  REPEAT_N 11 STRIP_TAC THEN
+  CONJ_TAC THENL [
+    ASM_MESON_TAC [STEPS_ADD; seq];
+    REPEAT STRIP_TAC THEN
+    DISJ_CASES_TAC (ARITH_RULE `n' < n1 \/ n' >= n1`) THENL [
+      ASM_MESON_TAC [];
+      FIRST_X_ASSUM (fun th -> CHOOSE_THEN ASSUME_TAC (REWRITE_RULE [GE; LE_EXISTS] th)) THEN
+      ASM_MESON_TAC [LT_ADD_LCANCEL; STEPS_ADD]]]);;
+
+let ENSURES_N_TRANS_SIMPLE = prove(
+  `!step (P:S->bool) (Q:S->bool) (R:S->bool) C n1 n2.
+    C ,, C = C /\
+    ensures_n step P Q C (\s. n1) /\ ensures_n step Q R C (\s. n2)
+    ==> ensures_n step P R C (\s. n1 + n2)`,
+  MESON_TAC[ENSURES_N_TRANS]);;
+
+let ENSURES_N_SEQUENCE_TAC =
+  let pth = prove
+   (`!program_decodes pcounter pc' Q n1 n2.
+        C ,, C = C /\
+        ensures_n step (\s. program_decodes s /\
+                          read pcounter s = word pc'' /\
+                          P s)
+                       (\s. program_decodes s /\
+                          read pcounter s = word pc' /\
+                          Q s)
+                       C (\s. n1) /\
+        ensures_n step (\s. program_decodes s /\
+                          read pcounter s = word pc' /\
+                          Q s)
+                       R C (\s. n2)
+        ==> ensures_n step (\s. program_decodes s /\
+                              read pcounter s = word pc'' /\
+                              P s)
+                           R C (\s. n1 + n2)`,
+    REWRITE_TAC[ENSURES_N_TRANS_SIMPLE]) in
+  let tac = MATCH_MP_TAC pth in
+  fun n q -> (tac THEN MAP_EVERY EXISTS_TAC [n;q] THEN BETA_TAC THEN
+              CONJ_TAC THENL [MAYCHANGE_IDEMPOT_TAC; ALL_TAC]);;
+
+(* ------------------------------------------------------------------------- *)
+(* Induction, basically a variant of the usual WHILE rule with a             *)
+(* test at the end. Versions for up from 0...k-1, down from k-1...0 and up   *)
+(* from a...b-1.                                                             *)
+(* ------------------------------------------------------------------------- *)
+
+let ENSURES_N_WHILE_UP_TAC, ENSURES_N_WHILE_DOWN_TAC,
+    ENSURES_N_WHILE_AUP_TAC, ENSURES_N_WHILE_ADOWN_TAC =
+  let pth = prove(
+    `!k pc1 pc2 (loopinvariant:num->A->bool) nsteps_pre f_nsteps nsteps_back nsteps_post.
+      C ,, C = C /\ ~(k = 0) /\
+      ensures_n step
+        (\s. program_decodes s /\ read pcounter s = word pc /\ precondition s)
+        (\s. program_decodes s /\ read pcounter s = word pc1 /\ loopinvariant 0 s)
+        C (\s. nsteps_pre) /\
+      (!i. i < k /\ ~(i = k) /\ ~(k = 0) /\ 0 < k
+        ==>
+        ensures_n step
+          (\s. program_decodes s /\ read pcounter s = word pc1 /\ loopinvariant i s)
+          (\s. program_decodes s /\ read pcounter s = word pc2 /\ loopinvariant (i + 1) s)
+          C (\s. f_nsteps i)) /\
+      (!i. 0 < i /\ i < k /\ ~(i = k) /\ ~(i = 0) /\ ~(k = 0) /\ 0 < k
+        ==>
+        ensures_n step
+          (\s. program_decodes s /\ read pcounter s = word pc2 /\ loopinvariant i s)
+          (\s. program_decodes s /\ read pcounter s = word pc1 /\ loopinvariant i s)
+          C (\s. nsteps_back)) /\
+      ensures_n step
+          (\s. program_decodes s /\ read pcounter s = word pc2 /\ loopinvariant k s)
+          postcondition C (\s. nsteps_post) /\
+      nsteps = nsteps_pre + (nsum (0..(k-1)) (\i. f_nsteps i) + (k-1) * nsteps_back) + nsteps_post
+      ==>
+      ensures_n step
+        (\s. program_decodes s /\ read pcounter s = word pc /\ precondition s)
+        postcondition C (\s. nsteps)`,
+    REPEAT STRIP_TAC THEN
+    CHOOSE_THEN ASSUME_TAC (GSYM (ISPEC `nsum (0..(k-1)) (\i. f_nsteps i) + (k-1) * nsteps_back` EXISTS_REFL)) THEN
+    IMP_REWRITE_TAC [ENSURES_N_TRANS_SIMPLE] THEN
+    UNDISCH_THEN `nsum (0..k - 1) (\i. f_nsteps i) + (k - 1) * nsteps_back = x` (fun th -> REWRITE_TAC [SYM th]) THEN
+    FIRST_ASSUM (SUBST1_TAC o MATCH_MP (ARITH_RULE `~(k = 0) ==> k = (k - 1) + 1`)) THEN
+    UNDISCH_THEN `~(k = 0)` (MP_TAC o MATCH_MP (ARITH_RULE `~(k = 0) ==> k - 1 < k`)) THEN
+    SPEC_TAC (`k-1:num`,`j:num`) THEN
+    REWRITE_TAC [ARITH_RULE `(j + 1) - 1 = j`] THEN
+    INDUCT_TAC THENL [
+      STRIP_TAC THEN REWRITE_TAC [NSUM_SING_NUMSEG; ADD_0; MULT] THEN
+      FIRST_X_ASSUM (MATCH_MP_TAC o SPEC `0`) THEN ASM_ARITH_TAC;
+      ASM_REWRITE_TAC [NSUM_CLAUSES_NUMSEG; ADD1; ARITH_RULE `0 <= j + 1`] THEN
+      ASM_REWRITE_TAC [ARITH_RULE `(nsum (0..j) (\i. f_nsteps i) + f_nsteps (j + 1)) + (j + 1) * nsteps_back = (nsum (0..j) (\i. f_nsteps i) + (j * nsteps_back)) + f_nsteps (j + 1) + nsteps_back`] THEN
+      STRIP_TAC THEN
+      MATCH_MP_TAC ENSURES_N_TRANS_SIMPLE THEN META_EXISTS_TAC THEN
+      ASM_REWRITE_TAC [] THEN
+      CONJ_TAC THENL [
+        UNDISCH_THEN `j + 1 < k` (MP_TAC o MP (ARITH_RULE `j + 1 < k ==> j < k`)) THEN
+        FIRST_X_ASSUM (UNIFY_ACCEPT_TAC [`Q:A->bool`]);
+        SUBST1_TAC (ARITH_RULE `f_nsteps (j + 1) + nsteps_back = nsteps_back + f_nsteps (j + 1)`) THEN
+        MATCH_MP_TAC ENSURES_N_TRANS_SIMPLE THEN META_EXISTS_TAC THEN
+        ASM_REWRITE_TAC [] THEN
+        CONJ_TAC THENL [
+          UNDISCH_THEN `j + 1 < k` (MP_TAC o MP (ARITH_RULE `j + 1 < k ==> 0 < j + 1 /\ j + 1 < k /\ ~(j + 1 = k) /\ ~(j + 1 = 0) /\ ~(k = 0) /\ 0 < k`)) THEN
+          FIRST_X_ASSUM (UNIFY_ACCEPT_TAC [`Q:A->bool`] o SPEC `j + 1`);
+          UNDISCH_THEN `j + 1 < k` (MP_TAC o MP (ARITH_RULE `j + 1 < k ==> j + 1 < k /\ ~(j + 1 = k) /\ ~(k = 0) /\ 0 < k`)) THEN
+          FIRST_X_ASSUM (UNIFY_ACCEPT_TAC [`Q:A->bool`] o SPEC `j + 1`)]]]) in
+  let qth = prove(
+    `!k pc1 pc2 (loopinvariant:num->A->bool) nsteps_pre f_nsteps nsteps_back nsteps_post.
+      C ,, C = C /\ ~(k = 0) /\
+      ensures_n step
+        (\s. program_decodes s /\ read pcounter s = word pc /\ precondition s)
+        (\s. program_decodes s /\ read pcounter s = word pc1 /\ loopinvariant k s)
+        C (\s. nsteps_pre) /\
+      (!i. i < k /\ ~(i = k) /\ ~(k = 0) /\ 0 < k
+        ==>
+        ensures_n step
+          (\s. program_decodes s /\ read pcounter s = word pc1 /\ loopinvariant (i + 1) s)
+          (\s. program_decodes s /\ read pcounter s = word pc2 /\ loopinvariant i s)
+          C (\s. f_nsteps i)) /\
+      (!i. 0 < i /\ i < k /\ ~(i = k) /\ ~(i = 0) /\ ~(k = 0) /\ 0 < k
+        ==>
+        ensures_n step
+          (\s. program_decodes s /\ read pcounter s = word pc2 /\ loopinvariant i s)
+          (\s. program_decodes s /\ read pcounter s = word pc1 /\ loopinvariant i s)
+          C (\s. nsteps_back)) /\
+      ensures_n step
+        (\s. program_decodes s /\ read pcounter s = word pc2 /\ loopinvariant 0 s)
+        postcondition C (\s. nsteps_post) /\
+      nsteps = nsteps_pre + (nsum (0..(k-1)) (\i. f_nsteps i) + (k-1) * nsteps_back) + nsteps_post
+      ==>
+      ensures_n step
+        (\s. program_decodes s /\ read pcounter s = word pc /\ precondition s)
+        postcondition C (\s. nsteps)`,
+    REPEAT GEN_TAC THEN DISCH_TAC THEN MATCH_MP_TAC pth THEN
+    MAP_EVERY EXISTS_TAC [`k:num`; `pc1:num`; `pc2:num`; `\i. (loopinvariant:num->A->bool) (k - i)`; `nsteps_pre:num`; `\i. (f_nsteps:num->num) (k - (i + 1))`; `nsteps_back:num`; `nsteps_post:num`] THEN
+    POP_ASSUM MP_TAC THEN REWRITE_TAC[SUB_0; SUB_REFL] THEN
+    REPEAT (MATCH_MP_TAC MONO_AND THEN CONJ_TAC THEN REWRITE_TAC[]) THENL [
+      DISCH_TAC THEN X_GEN_TAC `i:num` THEN DISCH_TAC THEN
+      FIRST_X_ASSUM (MP_TAC o SPEC `k - (i + 1)`) THEN
+      ASM_SIMP_TAC [ARITH_RULE `i < k ==> k - (i + 1) + 1 = k - i`] THEN
+      DISCH_THEN MATCH_MP_TAC THEN ASM_ARITH_TAC;
+      DISCH_TAC THEN X_GEN_TAC `i:num` THEN DISCH_TAC THEN
+      FIRST_X_ASSUM MATCH_MP_TAC THEN ASM_ARITH_TAC;
+      ASM_REWRITE_TAC [ARITH_RULE `k - (i + 1) = (k - 1) - i`; NSUM_REFLECT'; ETA_AX]]) in
+  let rth = prove(
+    `!a b pc1 pc2 (loopinvariant:num->A->bool) nsteps_pre f_nsteps nsteps_back nsteps_post.
+      C ,, C = C /\ a < b /\
+      ensures_n step
+        (\s. program_decodes s /\ read pcounter s = word pc /\ precondition s)
+        (\s. program_decodes s /\ read pcounter s = word pc1 /\ loopinvariant a s)
+        C (\s. nsteps_pre) /\
+      (!i. a <= i /\ i < b /\ ~(i = b) /\ ~(b = 0) /\ 0 < b
+        ==>
+        ensures_n step
+          (\s. program_decodes s /\ read pcounter s = word pc1 /\ loopinvariant i s)
+          (\s. program_decodes s /\ read pcounter s = word pc2 /\ loopinvariant (i + 1) s)
+          C (\s. f_nsteps i)) /\
+      (!i. a < i /\ i < b /\ ~(i = b) /\ ~(i = 0) /\ ~(i = a) /\ ~(b = 0) /\ 0 < b
+        ==>
+        ensures_n step
+          (\s. program_decodes s /\ read pcounter s = word pc2 /\ loopinvariant i s)
+          (\s. program_decodes s /\ read pcounter s = word pc1 /\ loopinvariant i s)
+          C (\s. nsteps_back)) /\
+      ensures_n step
+        (\s. program_decodes s /\ read pcounter s = word pc2 /\ loopinvariant b s)
+        postcondition C (\s. nsteps_post) /\
+      nsteps = nsteps_pre + (nsum(a..(b-1)) (\i. f_nsteps i) + (b-1-a) * nsteps_back) + nsteps_post
+      ==>
+      ensures_n step
+        (\s. program_decodes s /\ read pcounter s = word pc /\ precondition s)
+        postcondition C (\s. nsteps)`,
+    REPEAT STRIP_TAC THEN MATCH_MP_TAC pth THEN
+    MAP_EVERY EXISTS_TAC [`b - a:num`; `pc1:num`; `pc2:num`; `\i. (loopinvariant:num->A->bool) (a + i)`; `nsteps_pre:num`; `\i. (f_nsteps:num->num) (a + i)`; `nsteps_back:num`; `nsteps_post:num`] THEN
+    ASM_REWRITE_TAC [SUB_EQ_0; NOT_LE; ADD_CLAUSES] THEN
+    ASM_SIMP_TAC [ARITH_RULE `a:num < b ==> a + b - a = b`] THEN
+    REWRITE_TAC [ADD_ASSOC] THEN REPEAT STRIP_TAC THENL [
+      FIRST_X_ASSUM MATCH_MP_TAC THEN ASM_ARITH_TAC;
+      FIRST_X_ASSUM MATCH_MP_TAC THEN ASM_ARITH_TAC;
+      REWRITE_TAC [ARITH_RULE `b - a - 1 = b - 1 - a`] THEN
+      ONCE_ASM_REWRITE_TAC [MATCH_MP NSUM_OFFSET_0 (MP (ARITH_RULE `a < b ==> a <= b - 1`) (ASSUME `a < b`))] THEN
+      ASM_REWRITE_TAC [ADD_SYM]]) in
+  let sth = prove(
+    `!a b pc1 pc2 (loopinvariant:num->A->bool) nsteps_pre f_nsteps nsteps_back nsteps_post.
+      C ,, C = C /\ a < b /\
+      ensures_n step
+        (\s. program_decodes s /\ read pcounter s = word pc /\ precondition s)
+        (\s. program_decodes s /\ read pcounter s = word pc1 /\ loopinvariant b s)
+        C (\s. nsteps_pre) /\
+      (!i. a <= i /\ i < b /\ ~(i = b) /\ ~(b = 0) /\ 0 < b
+        ==>
+        ensures_n step
+          (\s. program_decodes s /\ read pcounter s = word pc1 /\ loopinvariant (i + 1) s)
+          (\s. program_decodes s /\ read pcounter s = word pc2 /\ loopinvariant i s)
+          C (\s. f_nsteps i)) /\
+      (!i. a < i /\ i < b /\ ~(i = a) /\ ~(i = 0) /\ ~(i = b) /\ ~(b = 0) /\ 0 < b
+        ==>
+        ensures_n step
+          (\s. program_decodes s /\ read pcounter s = word pc2 /\ loopinvariant i s)
+          (\s. program_decodes s /\ read pcounter s = word pc1 /\ loopinvariant i s)
+          C (\s. nsteps_back)) /\
+      ensures_n step
+        (\s. program_decodes s /\ read pcounter s = word pc2 /\ loopinvariant a s)
+        postcondition C (\s. nsteps_post) /\
+      nsteps = nsteps_pre + (nsum(a..(b-1)) (\i. f_nsteps i) + (b-1-a) * nsteps_back) + nsteps_post
+      ==>
+      ensures_n step
+        (\s. program_decodes s /\ read pcounter s = word pc /\ precondition s)
+        postcondition C (\s. nsteps)`,
+    REPEAT STRIP_TAC THEN MATCH_MP_TAC qth THEN
+    MAP_EVERY EXISTS_TAC [`b - a:num`; `pc1:num`; `pc2:num`; `\i. (loopinvariant:num->A->bool) (a + i)`; `nsteps_pre:num`; `\i. (f_nsteps:num->num) (a + i)`; `nsteps_back:num`; `nsteps_post:num`] THEN
+    ASM_REWRITE_TAC [SUB_EQ_0; NOT_LE; ADD_CLAUSES] THEN
+    ASM_SIMP_TAC [ARITH_RULE `a:num < b ==> a + b - a = b`] THEN
+    REWRITE_TAC [ADD_ASSOC] THEN REPEAT STRIP_TAC THENL [
+      FIRST_X_ASSUM MATCH_MP_TAC THEN ASM_ARITH_TAC;
+      FIRST_X_ASSUM MATCH_MP_TAC THEN ASM_ARITH_TAC;
+      REWRITE_TAC [ARITH_RULE `b - a - 1 = b - 1 - a`] THEN
+      ONCE_ASM_REWRITE_TAC [MATCH_MP NSUM_OFFSET_0 (MP (ARITH_RULE `a < b ==> a <= b - 1`) (ASSUME `a < b`))] THEN
+      ASM_REWRITE_TAC [ADD_SYM]]) in
+  (fun k pc1 pc2 iv f_nsteps nsteps_pre nsteps_back nsteps_post ->
+    MATCH_MP_TAC pth THEN
+    MAP_EVERY EXISTS_TAC [k; pc1; pc2; iv; nsteps_pre; f_nsteps; nsteps_back; nsteps_post] THEN
+    BETA_TAC THEN
+    CONJ_TAC THENL [MAYCHANGE_IDEMPOT_TAC'; ALL_TAC]),
+  (fun k pc1 pc2 iv f_nsteps nsteps_pre nsteps_back nsteps_post ->
+    MATCH_MP_TAC qth THEN
+    MAP_EVERY EXISTS_TAC [k; pc1; pc2; iv; nsteps_pre; f_nsteps; nsteps_back; nsteps_post] THEN
+    BETA_TAC THEN
+    CONJ_TAC THENL [MAYCHANGE_IDEMPOT_TAC'; ALL_TAC]),
+  (fun a b pc1 pc2 iv f_nsteps nsteps_pre nsteps_back nsteps_post ->
+    MATCH_MP_TAC rth THEN
+    MAP_EVERY EXISTS_TAC [a; b; pc1; pc2; iv; nsteps_pre; f_nsteps; nsteps_back; nsteps_post] THEN
+    BETA_TAC THEN
+    CONJ_TAC THENL [MAYCHANGE_IDEMPOT_TAC'; ALL_TAC]),
+  (fun b a pc1 pc2 iv f_nsteps nsteps_pre nsteps_back nsteps_post ->
+    MATCH_MP_TAC sth THEN
+    MAP_EVERY EXISTS_TAC [a; b; pc1; pc2; iv; nsteps_pre; f_nsteps; nsteps_back; nsteps_post] THEN
+    BETA_TAC THEN
+    CONJ_TAC THENL [MAYCHANGE_IDEMPOT_TAC'; ALL_TAC]);;
+
+(* ------------------------------------------------------------------------- *)
+(* Variants where there is an extra conjunct in the end state that may       *)
+(* not hold at the outset of the zeroth iteration. This is mainly intended   *)
+(* for cases where the last arithmetic operation sets flags that are then    *)
+(* used to decide the branch.                                                *)
+(* ------------------------------------------------------------------------- *)
+
+let ENSURES_N_WHILE_PUP_TAC,ENSURES_N_WHILE_PDOWN_TAC,
+    ENSURES_N_WHILE_PAUP_TAC,ENSURES_N_WHILE_PADOWN_TAC =
+  let pth = prove(
+    `!k pc1 pc2 p (q:num->A->bool) nsteps_pre f_nsteps nsteps_post.
+      C ,, C = C /\ ~(k = 0) /\
+      ensures_n step
+        (\s. program_decodes s /\ read pcounter s = word pc /\ precondition s)
+        (\s. program_decodes s /\ read pcounter s = word pc1 /\ p 0 s)
+        C (\s. nsteps_pre) /\
+      (!i. i < k /\ ~(i = k) /\ ~(k = 0) /\ 0 < k
+        ==>
+        ensures_n step
+          (\s. program_decodes s /\ read pcounter s = word pc1 /\ p i s)
+          (\s. program_decodes s /\ read pcounter s = word pc2 /\ p (i + 1) s /\ q (i + 1) s)
+          C (\s. f_nsteps i)) /\
+      (!i. 0 < i /\ i < k /\ ~(i = k) /\ ~(i = 0) /\ ~(k = 0) /\ 0 < k
+        ==>
+        ensures_n step
+          (\s. program_decodes s /\ read pcounter s = word pc2 /\ p i s /\ q i s)
+          (\s. program_decodes s /\ read pcounter s = word pc1 /\ p i s)
+          C (\s. 1)) /\
+      ensures_n step
+          (\s. program_decodes s /\ read pcounter s = word pc2 /\ p k s /\ q k s)
+          postcondition C (\s. nsteps_post) /\
+      nsteps = nsteps_pre + (nsum (0..(k-1)) (\i. f_nsteps i) + (k-1)) + nsteps_post
+      ==>
+      ensures_n step
+        (\s. program_decodes s /\ read pcounter s = word pc /\ precondition s)
+        postcondition C (\s. nsteps)`,
+    REPEAT STRIP_TAC THEN
+    CHOOSE_THEN ASSUME_TAC (GSYM (ISPEC `nsum (0..(k-1)) (\i. f_nsteps i) + (k-1)` EXISTS_REFL)) THEN
+    IMP_REWRITE_TAC [ENSURES_N_TRANS_SIMPLE] THEN
+    UNDISCH_THEN `nsum (0..k - 1) (\i. f_nsteps i) + k - 1 = x` (fun th -> REWRITE_TAC [SYM th]) THEN
+    FIRST_ASSUM (SUBST1_TAC o MATCH_MP (ARITH_RULE `~(k = 0) ==> k = (k - 1) + 1`)) THEN
+    UNDISCH_THEN `~(k = 0)` (MP_TAC o MATCH_MP (ARITH_RULE `~(k = 0) ==> k - 1 < k`)) THEN
+    SPEC_TAC (`k-1:num`,`j:num`) THEN
+    REWRITE_TAC [ARITH_RULE `(j + 1) - 1 = j`] THEN
+    INDUCT_TAC THENL [
+      STRIP_TAC THEN REWRITE_TAC [NSUM_SING_NUMSEG; ADD_0] THEN
+      FIRST_X_ASSUM (MATCH_MP_TAC o SPEC `0`) THEN ASM_ARITH_TAC;
+      ASM_REWRITE_TAC [NSUM_CLAUSES_NUMSEG; ADD1; ARITH_RULE `0 <= j + 1`] THEN
+      ASM_REWRITE_TAC [ARITH_RULE `(nsum (0..j) (\i. f_nsteps i) + f_nsteps (j + 1)) + j + 1 = (nsum (0..j) (\i. f_nsteps i) + j) + f_nsteps (j + 1) + 1`] THEN
+      STRIP_TAC THEN
+      MATCH_MP_TAC ENSURES_N_TRANS_SIMPLE THEN META_EXISTS_TAC THEN
+      ASM_REWRITE_TAC [] THEN
+      CONJ_TAC THENL [
+        UNDISCH_THEN `j + 1 < k` (MP_TAC o MP (ARITH_RULE `j + 1 < k ==> j < k`)) THEN
+        FIRST_X_ASSUM (UNIFY_ACCEPT_TAC [`Q:A->bool`]);
+        SUBST1_TAC (ARITH_RULE `f_nsteps (j + 1) + 1 = 1 + f_nsteps (j + 1)`) THEN
+        MATCH_MP_TAC ENSURES_N_TRANS_SIMPLE THEN META_EXISTS_TAC THEN
+        ASM_REWRITE_TAC [] THEN
+        CONJ_TAC THENL [
+          UNDISCH_THEN `j + 1 < k` (MP_TAC o MP (ARITH_RULE `j + 1 < k ==> 0 < j + 1 /\ j + 1 < k /\ ~(j + 1 = k) /\ ~(j + 1 = 0) /\ ~(k = 0) /\ 0 < k`)) THEN
+          FIRST_X_ASSUM (UNIFY_ACCEPT_TAC [`Q:A->bool`] o SPEC `j + 1`);
+          UNDISCH_THEN `j + 1 < k` (MP_TAC o MP (ARITH_RULE `j + 1 < k ==> j + 1 < k /\ ~(j + 1 = k) /\ ~(k = 0) /\ 0 < k`)) THEN
+          FIRST_X_ASSUM (UNIFY_ACCEPT_TAC [`Q:A->bool`] o SPEC `j + 1`)]]]) in
+  let qth = prove(
+    `!k pc1 pc2 p (q:num->A->bool) nsteps_pre f_nsteps nsteps_post.
+      C ,, C = C /\ ~(k = 0) /\
+      ensures_n step
+        (\s. program_decodes s /\ read pcounter s = word pc /\ precondition s)
+        (\s. program_decodes s /\ read pcounter s = word pc1 /\ p k s)
+        C (\s. nsteps_pre) /\
+      (!i. i < k /\ ~(i = k) /\ ~(k = 0) /\ 0 < k
+        ==>
+        ensures_n step
+          (\s. program_decodes s /\ read pcounter s = word pc1 /\ p (i + 1) s)
+          (\s. program_decodes s /\ read pcounter s = word pc2 /\ p i s /\ q i s)
+          C (\s. f_nsteps i)) /\
+      (!i. 0 < i /\ i < k /\ ~(i = k) /\ ~(i = 0) /\ ~(k = 0) /\ 0 < k
+        ==>
+        ensures_n step
+          (\s. program_decodes s /\ read pcounter s = word pc2 /\ p i s /\ q i s)
+          (\s. program_decodes s /\ read pcounter s = word pc1 /\ p i s)
+          C (\s. 1)) /\
+      ensures_n step
+        (\s. program_decodes s /\ read pcounter s = word pc2 /\ p 0 s /\ q 0 s)
+        postcondition C (\s. nsteps_post) /\
+      nsteps = nsteps_pre + (nsum (0..(k-1)) (\i. f_nsteps i) + (k-1)) + nsteps_post
+      ==>
+      ensures_n step
+        (\s. program_decodes s /\ read pcounter s = word pc /\ precondition s)
+        postcondition C (\s. nsteps)`,
+    REPEAT GEN_TAC THEN DISCH_TAC THEN MATCH_MP_TAC pth THEN
+    MAP_EVERY EXISTS_TAC [`k:num`; `pc1:num`; `pc2:num`; `\i. (p:num->A->bool) (k - i)`; `\i. (q:num->A->bool) (k - i)`; `nsteps_pre:num`; `\i. (f_nsteps:num->num) (k - (i + 1))`; `nsteps_post:num`] THEN
+    POP_ASSUM MP_TAC THEN REWRITE_TAC[SUB_0; SUB_REFL] THEN
+    REPEAT (MATCH_MP_TAC MONO_AND THEN CONJ_TAC THEN REWRITE_TAC[]) THENL [
+      DISCH_TAC THEN X_GEN_TAC `i:num` THEN DISCH_TAC THEN
+      FIRST_X_ASSUM (MP_TAC o SPEC `k - (i + 1)`) THEN
+      ASM_SIMP_TAC [ARITH_RULE `i < k ==> k - (i + 1) + 1 = k - i`] THEN
+      DISCH_THEN MATCH_MP_TAC THEN ASM_ARITH_TAC;
+      DISCH_TAC THEN X_GEN_TAC `i:num` THEN DISCH_TAC THEN
+      FIRST_X_ASSUM MATCH_MP_TAC THEN ASM_ARITH_TAC;
+      ASM_REWRITE_TAC [ARITH_RULE `k - (i + 1) = (k - 1) - i`; NSUM_REFLECT'; ETA_AX]]) in
+  let rth = prove(
+    `!a b pc1 pc2 p (q:num->A->bool) nsteps_pre f_nsteps nsteps_post.
+      C ,, C = C /\ a < b /\
+      ensures_n step
+        (\s. program_decodes s /\ read pcounter s = word pc /\ precondition s)
+        (\s. program_decodes s /\ read pcounter s = word pc1 /\ p a s)
+        C (\s. nsteps_pre) /\
+      (!i. a <= i /\ i < b /\ ~(i = b) /\ ~(b = 0) /\ 0 < b
+        ==>
+        ensures_n step
+          (\s. program_decodes s /\ read pcounter s = word pc1 /\ p i s)
+          (\s. program_decodes s /\ read pcounter s = word pc2 /\ p (i + 1) s /\ q (i + 1) s)
+          C (\s. f_nsteps i)) /\
+      (!i. a < i /\ i < b /\ ~(i = b) /\ ~(i = 0) /\ ~(i = a) /\ ~(b = 0) /\ 0 < b
+        ==>
+        ensures_n step
+          (\s. program_decodes s /\ read pcounter s = word pc2 /\ p i s /\ q i s)
+          (\s. program_decodes s /\ read pcounter s = word pc1 /\ p i s)
+          C (\s. 1)) /\
+      ensures_n step
+        (\s. program_decodes s /\ read pcounter s = word pc2 /\ p b s /\ q b s)
+        postcondition C (\s. nsteps_post) /\
+      nsteps = nsteps_pre + (nsum(a..(b-1)) (\i. f_nsteps i) + (b-1-a)) + nsteps_post
+      ==>
+      ensures_n step
+        (\s. program_decodes s /\ read pcounter s = word pc /\ precondition s)
+        postcondition C (\s. nsteps)`,
+    REPEAT STRIP_TAC THEN MATCH_MP_TAC pth THEN
+    MAP_EVERY EXISTS_TAC [`b - a:num`; `pc1:num`; `pc2:num`; `\i. (p:num->A->bool) (a + i)`; `\i. (q:num->A->bool) (a + i)`; `nsteps_pre:num`; `\i. (f_nsteps:num->num) (a + i)`; `nsteps_post:num`] THEN
+    ASM_REWRITE_TAC [SUB_EQ_0; NOT_LE; ADD_CLAUSES] THEN
+    ASM_SIMP_TAC [ARITH_RULE `a:num < b ==> a + b - a = b`] THEN
+    REWRITE_TAC [ADD_ASSOC] THEN REPEAT STRIP_TAC THENL [
+      FIRST_X_ASSUM MATCH_MP_TAC THEN ASM_ARITH_TAC;
+      FIRST_X_ASSUM MATCH_MP_TAC THEN ASM_ARITH_TAC;
+      REWRITE_TAC [ARITH_RULE `b - a - 1 = b - 1 - a`] THEN
+      ONCE_ASM_REWRITE_TAC [MATCH_MP NSUM_OFFSET_0 (MP (ARITH_RULE `a < b ==> a <= b - 1`) (ASSUME `a < b`))] THEN
+      ASM_REWRITE_TAC [ADD_SYM]]) in
+  let sth = prove(
+    `!a b pc1 pc2 p (q:num->A->bool) nsteps_pre f_nsteps nsteps_post.
+      C ,, C = C /\ a < b /\
+      ensures_n step
+        (\s. program_decodes s /\ read pcounter s = word pc /\ precondition s)
+        (\s. program_decodes s /\ read pcounter s = word pc1 /\ p b s)
+        C (\s. nsteps_pre) /\
+      (!i. a <= i /\ i < b /\ ~(i = b) /\ ~(b = 0) /\ 0 < b
+        ==>
+        ensures_n step
+          (\s. program_decodes s /\ read pcounter s = word pc1 /\ p (i + 1) s)
+          (\s. program_decodes s /\ read pcounter s = word pc2 /\ p i s /\ q i s)
+          C (\s. f_nsteps i)) /\
+      (!i. a < i /\ i < b /\ ~(i = a) /\ ~(i = 0) /\ ~(i = b) /\ ~(b = 0) /\ 0 < b
+        ==>
+        ensures_n step
+          (\s. program_decodes s /\ read pcounter s = word pc2 /\ p i s /\ q i s)
+          (\s. program_decodes s /\ read pcounter s = word pc1 /\ p i s)
+          C (\s. 1)) /\
+      ensures_n step
+        (\s. program_decodes s /\ read pcounter s = word pc2 /\ p a s /\ q a s)
+        postcondition C (\s. nsteps_post) /\
+      nsteps = nsteps_pre + (nsum(a..(b-1)) (\i. f_nsteps i) + (b-1-a)) + nsteps_post
+      ==>
+      ensures_n step
+        (\s. program_decodes s /\ read pcounter s = word pc /\ precondition s)
+        postcondition C (\s. nsteps)`,
+    REPEAT STRIP_TAC THEN MATCH_MP_TAC qth THEN
+    MAP_EVERY EXISTS_TAC [`b - a:num`; `pc1:num`; `pc2:num`; `\i. (p:num->A->bool) (a + i)`; `\i. (q:num->A->bool) (a + i)`; `nsteps_pre:num`; `\i. (f_nsteps:num->num) (a + i)`; `nsteps_post:num`] THEN
+    ASM_REWRITE_TAC [SUB_EQ_0; NOT_LE; ADD_CLAUSES] THEN
+    ASM_SIMP_TAC [ARITH_RULE `a:num < b ==> a + b - a = b`] THEN
+    REWRITE_TAC [ADD_ASSOC] THEN REPEAT STRIP_TAC THENL [
+      FIRST_X_ASSUM MATCH_MP_TAC THEN ASM_ARITH_TAC;
+      FIRST_X_ASSUM MATCH_MP_TAC THEN ASM_ARITH_TAC;
+      REWRITE_TAC [ARITH_RULE `b - a - 1 = b - 1 - a`] THEN
+      ONCE_ASM_REWRITE_TAC [MATCH_MP NSUM_OFFSET_0 (MP (ARITH_RULE `a < b ==> a <= b - 1`) (ASSUME `a < b`))] THEN
+      ASM_REWRITE_TAC [ADD_SYM]]) in
+  (fun k pc1 pc2 p q f_nsteps nsteps_pre nsteps_post ->
+    MATCH_MP_TAC pth THEN
+    MAP_EVERY EXISTS_TAC [k; pc1; pc2; p; q; nsteps_pre; f_nsteps; nsteps_post] THEN
+    BETA_TAC THEN
+    CONJ_TAC THENL [MAYCHANGE_IDEMPOT_TAC'; ALL_TAC]),
+  (fun k pc1 pc2 p q f_nsteps nsteps_pre nsteps_post ->
+    MATCH_MP_TAC qth THEN
+    MAP_EVERY EXISTS_TAC [k; pc1; pc2; p; q; nsteps_pre; f_nsteps; nsteps_post] THEN
+    BETA_TAC THEN
+    CONJ_TAC THENL [MAYCHANGE_IDEMPOT_TAC'; ALL_TAC]),
+  (fun a b pc1 pc2 p q f_nsteps nsteps_pre nsteps_post ->
+    MATCH_MP_TAC rth THEN
+    MAP_EVERY EXISTS_TAC [a; b; pc1; pc2; p; q; nsteps_pre; f_nsteps; nsteps_post] THEN
+    BETA_TAC THEN
+    CONJ_TAC THENL [MAYCHANGE_IDEMPOT_TAC'; ALL_TAC]),
+  (fun b a pc1 pc2 p q f_nsteps nsteps_pre nsteps_post ->
+    MATCH_MP_TAC sth THEN
+    MAP_EVERY EXISTS_TAC [a; b; pc1; pc2; p; q; nsteps_pre; f_nsteps; nsteps_post] THEN
+    BETA_TAC THEN
+    CONJ_TAC THENL [MAYCHANGE_IDEMPOT_TAC'; ALL_TAC]);;
+
+(* ------------------------------------------------------------------------- *)
+(* Introduce a new ghost variable for a state component in "ensures".        *)
+(* ------------------------------------------------------------------------- *)
+
+let GHOST_INTRO'_TAC =
+  let pth = prove
+   (`!f P step post frame fn.
+         (!a. ensures_n step (\s. P s a /\ f s = a) post frame fn)
+         ==> ensures_n step (\s. P s (f s)) post frame fn`,
+    REPEAT GEN_TAC THEN REWRITE_TAC[ensures_n] THEN
+    GEN_REWRITE_TAC LAND_CONV [SWAP_FORALL_THM] THEN
+    REWRITE_TAC[IMP_CONJ_ALT; FORALL_UNWIND_THM1]) in
+  fun t comp ->
+    MP_TAC(ISPEC comp pth) THEN
+    CONV_TAC(LAND_CONV(ONCE_DEPTH_CONV BETA_CONV)) THEN
+    DISCH_THEN MATCH_MP_TAC THEN X_GEN_TAC t THEN
+    GEN_REWRITE_TAC (RATOR_CONV o LAND_CONV o ABS_CONV o TOP_DEPTH_CONV)
+     [GSYM CONJ_ASSOC];;
+
+(* ------------------------------------------------------------------------- *)
+(* A way of using a lemma for a subroutine or subcomponent.                  *)
+(* Tactic supports the basic templating and leaves two user subgoals.        *)
+(* ------------------------------------------------------------------------- *)
+
+let ENSURES_N_SUBLEMMA_THM = prove
+ (`!t (P:A->bool) Q R.
+        (!s. P s ==> P' s) /\
+        R' subsumed R /\
+        (!s s'. P s /\ Q' s' /\ R' s s' ==> Q s')
+        ==> ensures t P' Q' R' ==> ensures t P Q R`,
+  REPEAT GEN_TAC THEN REWRITE_TAC[subsumed] THEN STRIP_TAC THEN
+  REWRITE_TAC[ensures] THEN MATCH_MP_TAC MONO_FORALL THEN
+  X_GEN_TAC `s:A` THEN DISCH_THEN(fun th -> DISCH_TAC THEN MP_TAC th) THEN
+  ASM_SIMP_TAC[] THEN
+  MATCH_MP_TAC(REWRITE_RULE[RIGHT_IMP_FORALL_THM]
+        EVENTUALLY_MONO) THEN
+  ASM_MESON_TAC[]);;
+
+let ENSURES_SUBLEMMA_TAC execth s0 s1 =
+  MATCH_MP_TAC ENSURES_SUBLEMMA_THM THEN
+  REWRITE_TAC[] THEN CONJ_TAC THENL
+   [W(fun (asl,w) -> X_GEN_TAC(mk_var(s0,type_of(fst(dest_forall w))))) THEN
+    STRIP_TAC;
+    CONJ_TAC THENL [SUBSUMED_MAYCHANGE_TAC THEN NO_TAC; ALL_TAC] THEN
+    W(fun (asl,w) -> X_GEN_TAC(mk_var(s0,type_of(fst(dest_forall w))))) THEN
+    W(fun (asl,w) -> X_GEN_TAC(mk_var(s1,type_of(fst(dest_forall w))))) THEN
+    REPEAT(DISCH_THEN(CONJUNCTS_THEN2 STRIP_ASSUME_TAC MP_TAC)) THEN
+    REWRITE_TAC[MAYCHANGE; SEQ_ID] THEN
+    REWRITE_TAC[GSYM SEQ_ASSOC] THEN
+    REWRITE_TAC[ASSIGNS_SEQ] THEN REWRITE_TAC[ASSIGNS_THM] THEN
+    REWRITE_TAC[LEFT_IMP_EXISTS_THM] THEN REPEAT GEN_TAC THEN
+    NONSELFMODIFYING_STATE_UPDATE_TAC execth THEN
+    ASSUMPTION_STATE_UPDATE_TAC THEN DISCH_THEN(K ALL_TAC)];;
+
+(*** A version that also tries nonmodification for subroutines ***)
+
+let ENSURES_SUBSUBLEMMA_TAC (execth::subths) s0 s1 =
+  MATCH_MP_TAC ENSURES_SUBLEMMA_THM THEN
+  REWRITE_TAC[] THEN CONJ_TAC THENL
+   [W(fun (asl,w) -> X_GEN_TAC(mk_var(s0,type_of(fst(dest_forall w))))) THEN
+    STRIP_TAC;
+    CONJ_TAC THENL [SUBSUMED_MAYCHANGE_TAC THEN NO_TAC; ALL_TAC] THEN
+    W(fun (asl,w) -> X_GEN_TAC(mk_var(s0,type_of(fst(dest_forall w))))) THEN
+    W(fun (asl,w) -> X_GEN_TAC(mk_var(s1,type_of(fst(dest_forall w))))) THEN
+    REPEAT(DISCH_THEN(CONJUNCTS_THEN2 STRIP_ASSUME_TAC MP_TAC)) THEN
+    REWRITE_TAC[MAYCHANGE; SEQ_ID] THEN
+    REWRITE_TAC[GSYM SEQ_ASSOC] THEN
+    REWRITE_TAC[ASSIGNS_SEQ] THEN REWRITE_TAC[ASSIGNS_THM] THEN
+    REWRITE_TAC[LEFT_IMP_EXISTS_THM] THEN REPEAT GEN_TAC THEN
+    NONSELFMODIFYING_STATE_UPDATE_TAC execth THEN
+    MAP_EVERY (TRY o NONSELFMODIFYING_STATE_UPDATE_TAC) subths THEN
+    ASSUMPTION_STATE_UPDATE_TAC THEN DISCH_THEN(K ALL_TAC)];;
+
+(* ------------------------------------------------------------------------- *)
+(* A way of using a lemma for a subroutine or subcomponent.                  *)
+(* Tactic supports the basic templating and leaves two user subgoals.        *)
+(* ------------------------------------------------------------------------- *)
+
+let ENSURES_N_SUBLEMMA_THM = prove
+  (`!t (P:A->bool) Q R fn.
+         (!s. P s ==> P' s) /\
+         R' subsumed R /\
+         (!s s'. P s /\ Q' s' /\ R' s s' ==> Q s')
+         ==> ensures_n t P' Q' R' fn ==> ensures_n t P Q R fn`,
+   REPEAT GEN_TAC THEN REWRITE_TAC[subsumed] THEN STRIP_TAC THEN
+   REWRITE_TAC[ensures_n] THEN MATCH_MP_TAC MONO_FORALL THEN
+   X_GEN_TAC `s:A` THEN DISCH_THEN(fun th -> DISCH_TAC THEN MP_TAC th) THEN
+   ASM_SIMP_TAC[] THEN
+   MATCH_MP_TAC(REWRITE_RULE[RIGHT_IMP_FORALL_THM]
+         EVENTUALLY_N_MONO) THEN
+   ASM_MESON_TAC[]);;
+
+let ENSURES_N_ENSURES_TAC th =
+  REPEAT GEN_TAC THEN REPEAT DISCH_TAC THEN
+  MATCH_MP_TAC ENSURES_N_ENSURES THEN META_EXISTS_TAC THEN
+  MP_TAC (SPEC_ALL th) THEN ASM_REWRITE_TAC[] THEN
+  DISCH_THEN (UNIFY_ACCEPT_TAC [`f_n:armstate->num`]);;
+
+(* ------------------------------------------------------------------------- *)
+(* Scrub a "preserved" component from the MAYCHANGE list.                    *)
+(* ------------------------------------------------------------------------- *)
+
+let ENSURES_N_MAYCHANGE_PRESERVED = prove
+ (`!(c:(A,B)component) t P Q R fn.
+        extensionally_valid_component c /\
+        (!s s'. R s s' ==> read c s' = read c s) /\
+        (!d. ensures_n t (\s. P s /\ read c s = d)
+                       (\s. Q s /\ read c s = d)
+                       (R ,, MAYCHANGE [c]) fn)
+        ==> ensures_n t P Q R fn`,
+  REPEAT GEN_TAC THEN REWRITE_TAC[ensures_n; EXTENSIONALLY_VALID_COMPONENT] THEN
+  STRIP_TAC THEN X_GEN_TAC `s0:A` THEN DISCH_TAC THEN
+  ABBREV_TAC `d = read (c:(A,B)component) s0` THEN
+  FIRST_X_ASSUM(MP_TAC o SPECL [`d:B`; `s0:A`]) THEN
+  ASM_REWRITE_TAC[MAYCHANGE; SEQ_ID] THEN
+  REWRITE_TAC[ASSIGNS_THM; seq] THEN
+  FIRST_X_ASSUM(MP_TAC o SPEC `s0:A`) THEN
+  ABBREV_TAC `fr = (R:A->A->bool) s0` THEN DISCH_TAC THEN
+  SPEC_TAC(`(fn:A->num) s0`,`n:num`) THEN SPEC_TAC(`s0:A`,`s0:A`) THEN
+  MATCH_MP_TAC EVENTUALLY_N_MONO2 THEN
+  X_GEN_TAC `s2:A` THEN REWRITE_TAC[] THEN
+  DISCH_THEN(CONJUNCTS_THEN2 STRIP_ASSUME_TAC MP_TAC) THEN
+  ASM_REWRITE_TAC[LEFT_IMP_EXISTS_THM] THEN
+  X_GEN_TAC `s1:A` THEN DISCH_THEN(CONJUNCTS_THEN2 ASSUME_TAC MP_TAC) THEN
+  DISCH_THEN(X_CHOOSE_TAC `y:B`) THEN
+  ASM_MESON_TAC[]);;
+
+let ENSURES_N_PRESERVED_TAC pname ctm =
+  MATCH_MP_TAC(ISPEC ctm ENSURES_N_MAYCHANGE_PRESERVED) THEN
+  CONJ_TAC THENL [CONV_TAC EXTENSIONALLY_VALID_COMPONENT_CONV; ALL_TAC] THEN
+  REWRITE_TAC[] THEN CONJ_TAC THENL
+   [REWRITE_TAC[MAYCHANGE; SEQ_ID] THEN
+    REWRITE_TAC[GSYM SEQ_ASSOC] THEN
+    REWRITE_TAC[ASSIGNS_SEQ] THEN REWRITE_TAC[ASSIGNS_THM] THEN
+    REWRITE_TAC[LEFT_IMP_EXISTS_THM] THEN REPEAT GEN_TAC THEN
+    DISCH_THEN(SUBST1_TAC o SYM) THEN
+    CONV_TAC(LAND_CONV(DEPTH_CONV
+     COMPONENT_READ_OVER_WRITE_ORTHOGONAL_CONV)) THEN
+    REFL_TAC;
+    REWRITE_TAC[GSYM CONJ_ASSOC; GSYM SEQ_ASSOC] THEN
+    W(fun (asl,w) -> X_GEN_TAC(mk_var(pname,type_of(fst(dest_forall w)))))];;
+
+let ENSURES_N_MAYCHANGE_EXISTING_PRESERVED = prove
+ (`!(c:(A,B)component) d t P Q R fn.
+        extensionally_valid_component c /\
+        (!s s'. R s s' ==> read c s' = read c s) /\
+        (!s. P s ==> read c s = d) /\
+        ensures_n t P (\s. Q s /\ read c s = d) (R ,, MAYCHANGE [c]) fn
+        ==> ensures_n t P Q R fn`,
+  REPEAT STRIP_TAC THEN MATCH_MP_TAC ENSURES_N_MAYCHANGE_PRESERVED THEN
+  EXISTS_TAC `c:(A,B)component` THEN ASM_REWRITE_TAC[] THEN
+  ONCE_REWRITE_TAC[TAUT `p /\ q <=> ~(p ==> ~q)`] THEN
+  ASM_SIMP_TAC[] THEN X_GEN_TAC `e:B` THEN
+  ASM_CASES_TAC `e:B = d` THEN
+  ASM_REWRITE_TAC[NOT_IMP; ENSURES_N_TRIVIAL; ETA_AX]);;
+
+let ENSURES_N_EXISTING_PRESERVED_TAC ctm =
+  W(fun (asl,w) ->
+        MATCH_MP_TAC(ISPEC ctm ENSURES_N_MAYCHANGE_EXISTING_PRESERVED) THEN
+        EXISTS_TAC(rand(find (fun e -> is_eq e && free_in ctm (lhand e))
+                             (conjuncts(body(lhand(rator w))))))) THEN
+  CONJ_TAC THENL [CONV_TAC EXTENSIONALLY_VALID_COMPONENT_CONV; ALL_TAC] THEN
+  REWRITE_TAC[] THEN CONJ_TAC THENL
+   [REWRITE_TAC[MAYCHANGE; SEQ_ID] THEN
+    REWRITE_TAC[GSYM SEQ_ASSOC] THEN
+    REWRITE_TAC[ASSIGNS_SEQ] THEN REWRITE_TAC[ASSIGNS_THM] THEN
+    REWRITE_TAC[LEFT_IMP_EXISTS_THM] THEN REPEAT GEN_TAC THEN
+    DISCH_THEN(SUBST1_TAC o SYM) THEN
+    CONV_TAC(LAND_CONV(DEPTH_CONV
+     COMPONENT_READ_OVER_WRITE_ORTHOGONAL_CONV)) THEN
+    REFL_TAC;
+    ALL_TAC] THEN
+  CONJ_TAC THENL
+   [REPEAT STRIP_TAC THEN ASM_REWRITE_TAC[] THEN NO_TAC;
+    REWRITE_TAC[GSYM CONJ_ASSOC; GSYM SEQ_ASSOC]];;
+
+
+(* ------------------------------------------------------------------------- *)
+(* Refinment of ENSURES_PRESERVED_TAC for special D register handling.       *)
+(* ------------------------------------------------------------------------- *)
+
+let ENSURES_N_PRESERVED_DREG_TAC =
+  let pth = prove
+   (`read (Q8 :> bottomhalf) s = word_zx(read Q8 s) /\
+     read (Q9 :> bottomhalf) s = word_zx (read Q9 s) /\
+     read (Q10 :> bottomhalf) s = word_zx (read Q10 s) /\
+     read (Q11 :> bottomhalf) s = word_zx (read Q11 s) /\
+     read (Q12 :> bottomhalf) s = word_zx (read Q12 s) /\
+     read (Q13 :> bottomhalf) s = word_zx (read Q13 s) /\
+     read (Q14 :> bottomhalf) s = word_zx (read Q14 s) /\
+     read (Q15 :> bottomhalf) s = word_zx (read Q15 s)`,
+    CONV_TAC(ONCE_DEPTH_CONV COMPONENT_CANON_CONV) THEN
+    REWRITE_TAC[READ_COMPONENT_COMPOSE; READ_ZEROTOP_64;
+                bottomhalf; subword; read; FUN_EQ_THM] THEN
+    REWRITE_TAC[word_zx; DIV_1; EXP; WORD_MOD_SIZE])
+  and sth = prove
+   (`valid_component c /\
+     R ,, R = R /\
+     MAYCHANGE [c :> tophalf] subsumed R /\
+     ensures_n step P Q (R ,, MAYCHANGE [c]) fn
+     ==> ensures_n step P Q (R ,, MAYCHANGE [c :> bottomhalf]) fn`,
+    REWRITE_TAC[MAYCHANGE_SING] THEN
+    REPEAT(DISCH_THEN(CONJUNCTS_THEN2 ASSUME_TAC MP_TAC)) THEN
+    MATCH_MP_TAC(REWRITE_RULE[IMP_CONJ] ENSURES_N_FRAME_SUBSUMED) THEN
+    FIRST_ASSUM(fun th ->
+      GEN_REWRITE_TAC (RAND_CONV o ONCE_DEPTH_CONV) [SYM th]) THEN
+    REWRITE_TAC[GSYM SEQ_ASSOC] THEN MATCH_MP_TAC SUBSUMED_SEQ THEN
+    REWRITE_TAC[SUBSUMED_REFL] THEN
+    FIRST_ASSUM(SUBST1_TAC o SYM o MATCH_MP ASSIGNS_TOPHALF_BOTTOMHALF) THEN
+    MATCH_MP_TAC SUBSUMED_SEQ THEN ASM_REWRITE_TAC[SUBSUMED_REFL]) in
+  let alist = zip [`D8`; `D9`; `D10`; `D11`; `D12`; `D13`; `D14`; `D15`]
+                  (map (lhand o lhand o concl) (CONJUNCTS pth)) in
+  let dregs = map fst alist in
+  fun pname ctm ->
+    if not (mem ctm dregs) then ENSURES_N_PRESERVED_TAC pname ctm else
+    let ctm' = assoc ctm alist in
+    ENSURES_N_PRESERVED_TAC pname ctm' THEN REWRITE_TAC[pth] THEN
+    TRY(REWRITE_TAC[SEQ_ASSOC] THEN MATCH_MP_TAC sth THEN
+        CONJ_TAC THENL [CONV_TAC VALID_COMPONENT_CONV; ALL_TAC] THEN
+        CONJ_TAC THENL [MAYCHANGE_IDEMPOT_TAC; ALL_TAC] THEN
+        CONJ_TAC THENL [SUBSUMED_MAYCHANGE_TAC THEN NO_TAC; ALL_TAC] THEN
+        REWRITE_TAC[GSYM SEQ_ASSOC]);;
